Multi-model complexity

src/lambda_calculus/utlc/beta/basic.lean
@@ -10,7 +10,6 @@ local notation a `[` b `:=` c  `]` : 70 := has_substitution.substitution a b c
 
 variables {f g f' g' x y z: utlc}
 
-@[simp]
 def head_step : utlc → utlc → Prop
 | (↓ _) := λ g, false
 | (Λ _) := λ g, false
@@ -20,90 +19,106 @@ def head_step : utlc → utlc → Prop
   | (_ · _) := λ g, false
   end
 
+section
+local attribute [simp] head_step
+
 instance head_step.decidable_rel : decidable_rel head_step :=
 begin
   intros f _,
-  cases f,
-  any_goals { simp [head_step], apply_instance },
-  cases f_f,
-  all_goals { simp [head_step], apply_instance },
+  cases f;
+  try { cases f_f };
+  { simp, apply_instance }
 end
 
-@[simp] theorem lambda_head_step:
-  head_step (Λ f) (Λ g) → head_step f g := by simp[head_step]
+theorem head_step_exists (f g: utlc): head_step f g ↔
+  ∃ x y, f = (Λ x)·y ∧ x[0:=y] = g :=
+by cases f; try { cases f_f }; simp [and.assoc]
+end
+attribute [simp] head_step_exists
+attribute [irreducible] head_step
 
 instance : has_β_reduction utlc := ⟨ reduction_step_of head_step ⟩
 
-@[simp] theorem lambda_step_iff:
-  (Λ f) →β (Λ g) ↔ f →β g :=
-begin
-  simp [has_β_reduction.step, reduction_step],
+section
+@[simp] theorem not_index_step (n: ℕ) (g: utlc): ¬ ↓n →β g := by simp [has_β_reduction.step]
+
+theorem lambda_step_iff (f g: utlc): Λ f →β g ↔ ∃ x, g = Λ x ∧ f →β x := by simp [has_β_reduction.step]
+
+theorem dot_step_iff (f f' g: utlc): f·f' →β g ↔
+  (∃ x, f = Λ x ∧ x[0:=f'] = g) ∨
+  (∃ x, g = x·f' ∧ f →β x) ∨
+  (∃ x, g = f·x ∧ f' →β x) := by simp [and.assoc, has_β_reduction.step]
 end
 
-theorem dot_step_dot_left (g: utlc): f →β f' → f·g →β f'·g :=
+theorem lambda_step_exists {f g: utlc}: Λ f →β g → ∃ x, g = Λ x ∧ f →β x := (lambda_step_iff _ _).mp
+
+theorem lambda_step_lambda {f g: utlc}: f →β g → Λ f →β Λ g :=
+by rw [lambda_step_iff]; intro p; exact ⟨g, rfl, p⟩
+
+@[simp] theorem lambda_step_lambda_iff {f g: utlc}: Λ f →β Λ g ↔ f →β g :=
+by simp [lambda_step_iff]
+
+@[simp] theorem step_index_iff (n: ℕ):
+  f →β ↓n ↔ f = (Λ ↓0)·↓n ∨ ∃ g, f = (Λ ↓(n+1))·g :=
 begin
-  intro p,
-  simp [has_β_reduction.step, reduction_step],
-  exact or.inr (or.inl p),
+  cases f;
+  try { cases f_f };
+  try { cases f_f };
+  try { cases f_f };
+  simp [and.assoc, lambda_step_iff, dot_step_iff, show 0 ≠ n + 1, by linarith, nat.succ_eq_add_one],
 end
 
-theorem dot_step_dot_right (f: utlc): g →β g' → f·g →β f·g' :=
-begin
-  intro p,
-  simp [has_β_reduction.step, reduction_step],
-  exact or.inr (or.inr p),
-end
+theorem dot_step_dot_left: f →β f' → ∀ g, f·g →β f'·g :=
+by intro p; simp [dot_step_iff]; exact λ _, or.inr (or.inl p)
+
+theorem dot_step_dot_right: g →β g' → ∀ f, f·g →β f·g' :=
+by intro p; simp [dot_step_iff]; exact λ _, or.inr (or.inr p)
+
+theorem dot_step_cases: f·f' →β g →
+  (∃ x, f = Λ x ∧ x[0:=f'] = g) ∨
+  (∃ x, g = x·f' ∧ f →β x) ∨
+  (∃ x, g = f·x ∧ f' →β x) := (dot_step_iff f f' g).mp
+
 
 theorem lambda_dot_step_substitution (f g: utlc):  (Λ f)·g →β f[0:=g] :=
-by simp [has_β_reduction.step, reduction_step]
+by simp [dot_step_iff]
+
+theorem down_dot_step_dot {n: ℕ}:
+  (↓n·x) →β (↓n·g) ↔ (x →β g) :=
+by simp [dot_step_iff]
+
+@[simp] theorem down_dot_step_dot' {n: ℕ}:
+  (↓n·x) →β (f·g) ↔ (f = ↓n) ∧ (x →β g) :=
+by simp [dot_step_iff, and.assoc]
 
 theorem dot_dot_step_dot:
-  (x·y·z) →β (f·g) → (x·y →β f ∧ z = g ∨ x·y=f ∧ z →β g) :=
+  (x·y·z) →β (f·g) → (x·y →β f ∧ z = g ∨ x·y = f ∧ z →β g) :=
 begin
-  intro a,
-  simp [has_β_reduction.step] at *,
-  rw [reduction_step] at a,
-  cases a,
-  { simp at a, contradiction },
-  any_goals { assumption },
+  intro h,
+  obtain h|h|h := dot_step_cases h;
+  try { { simp at h, contradiction } };
+  rcases h with ⟨w, hw, h⟩;
+  simp at hw;
+  rw [hw.left, hw.right],
+  exact or.inl ⟨h, rfl⟩,
+  exact or.inr ⟨rfl, h⟩
 end
 
-@[simp] theorem lambda_reduction_lambda:
-  f ↠β g → (Λ f) ↠β (Λ g) :=
-begin
-  intro _,
-  apply relation.refl_trans_gen.lift,
-  simp,
-  intros _ _ _,
-  assumption,
-  assumption
-end
+theorem lambda_reduction_lambda:
+  f ↠β g → (Λ f) ↠β (Λ g) := lambda_refl_trans_reduction_step_lambda
 
-@[simp] theorem dot_reduction_dot:
-  f ↠β g → f' ↠β g' → (f·f') ↠β (g·g') :=
-begin
-  intros _ _,
-  apply @trans _ _ _ _ (f·g'),
-  simp [show ∀ g, f·g = (λg, f·g) g, by simp],
-  apply relation.refl_trans_gen.lift,
-  intros _ _ _,
-  simp [has_β_reduction.step, reduction_step],
-  right,
-  right,
-  assumption,
-  assumption,
-  simp [show ∀ f, f·g' = (λf, f·g') f, by simp],
-  apply relation.refl_trans_gen.lift,
-  intros _ _ _,
-  simp [has_β_reduction.step, reduction_step],
-  right,
-  left,
-  assumption,
-  assumption,
-  apply_instance,
-end
+theorem dot_reduction_dot:
+  f ↠β g → f' ↠β g' → (f·f') ↠β (g·g') := dot_refl_trans_reduction_step_dot
 
-@[simp] theorem dot_reduction_substitution:
+theorem dot_reduction_dot_left:
+  f ↠β g → (f·f') ↠β (g·f') :=
+by intros p; apply dot_reduction_dot p; refl 
+
+theorem dot_reduction_dot_right:
+  f' ↠β g' → (f·f') ↠β (f·g') :=
+by apply dot_reduction_dot; refl
+
+theorem dot_reduction_substitution:
   f ↠β (Λ g) → f' ↠β g' → (f·f') ↠β g[0:=g'] :=
 begin
   intros _ _,
@@ -116,13 +131,54 @@ begin
   assumption,
   refl,
   apply relation.refl_trans_gen.single,
-  simp [has_β_reduction.step, reduction_step],
-  apply_instance,
-  apply_instance,
+  simp [dot_step_iff],
+  repeat { apply_instance }
 end
 
-@[simp]
-def head_reduced : utlc → bool
+theorem uses_zero_head_step: head_step f g → ∀ {n}, f.uses n = 0 → g.uses n = 0 :=
+begin
+  cases f;
+  simp,
+  intros x p q n hfx hxg,
+  simp [hxg, hfx, ← p, ← q, 
+    substitution_uses_zero (nat.zero_le n),
+    ← lambda_uses],
+end
+
+theorem uses_zero_step: f →β g → ∀ {n}, f.uses n = 0 → g.uses n = 0 := uses_zero_reduction_step @uses_zero_head_step
+
+theorem shift_head_step_shift {n: ℕ}: head_step (f ↑¹ n) (g ↑¹ n) ↔ head_step f g :=
+begin
+  cases f;
+  cases g;
+  try { { simp } };
+  cases f_f;
+  simp [and.assoc];
+  simp only [← down_shift, ← lambda_shift, ← dot_shift, ← substitution_shift_zero];
+  rw [shift_inj_iff],
+end
+
+theorem shift_head_step_shift' {n: ℕ}: head_step f g ↔ head_step (f ↑¹ n) (g ↑¹ n)  :=
+by rw [shift_head_step_shift]
+
+
+theorem shift_step_shift: f →β g → ∀ n, (f ↑¹ n) →β (g ↑¹ n) :=
+begin
+  simp [has_β_reduction.step],
+  intros p n,
+  rw [shift_reduction_step_shift_iff],
+  apply p,
+  apply shift_head_step_shift,
+end
+
+theorem shift_reduction_shift: f ↠β g → ∀ n, (f ↑¹ n) ↠β (g ↑¹ n) :=
+begin
+  simp [has_β_reduction.step],
+  intros p n,
+  apply shift_refl_trans_reduction_shift (@shift_head_step_shift) p
+end
+
+@[simp] def head_reduced : utlc → bool
 | (↓ _) := true
 | (Λ _) := true
 | (f·g) := match f with
@@ -131,53 +187,44 @@ def head_reduced : utlc → bool
   | (f·g) := true
   end
 
-@[simp]
-def reduced := λ f, lambda_calculus.utlc.reduced f head_reduced
+@[simp] def reduced := λ f, lambda_calculus.utlc.reduced_of head_reduced f
+
+theorem not_head_step_iff_head_reduced: head_reduced f ↔ ∀ g, ¬ head_step f g :=
+by cases f; try { cases f_f }; simp
 
 @[simp] theorem lambda_reduced_iff:
-  reduced (Λ f) ↔ reduced f := by simp [lambda_calculus.utlc.reduced]
+  reduced (Λ f) ↔ reduced f := by simp [lambda_reduced]
 
 theorem lambda_of_reduced_and_closed: reduced f → f.closed → ∃ g, f = Λ g :=
 begin
   induction f with _ f _ f g fh,
   { simp [closed, closed_below] },
-  { intros _ _,
-    use f,
-    refl },
-  simp [lambda_calculus.utlc.reduced, closed_below],
+  { intros _ _, use f, refl },
+  simp [closed_below],
   cases f with _ _ f f',
-  any_goals { { simp [lambda_calculus.utlc.reduced, closed_below] } },
+  any_goals { { simp [closed_below] } },
   intros _ p _ q _,
   specialize fh p q,
   simp at fh,
   contradiction
 end
 
+def reduced_of_not_reduction (f: utlc): reduced f ↔ ∀ g, ¬ f →β g :=
+  reduced_iff_not_reduction_step @not_head_step_iff_head_reduced _
 
-def not_reduction_of_reduced {f: utlc}: reduced f → ∀ g, ¬ f →β g :=
-begin
-  induction f,
-  all_goals { simp [has_β_reduction.step, reduction_step, lambda_calculus.utlc.reduced] },
-  { intros p g,
-    cases g,
-    all_goals { simp [has_β_reduction.step, reduction_step] },
-    exact f_ih p _ },
-  { intros p q r g,
-    cases g,
-    all_goals { simp [has_β_reduction.step, reduction_step] },
-    any_goals { intro h, cases h, revert h },
-    any_goals {
-      cases f_f,
-      any_goals { simp },
-      simp [lambda_calculus.utlc.reduced] at p,
-      contradiction },
-    { cases h,
-      all_goals { cases h },
-      specialize f_ih_f q g_f,
-      contradiction,
-      specialize f_ih_g r g_g,
-      contradiction } }
-end
+-- inductive hypothesis useful when dealing with β reductions
+-- splits f·g up to handle the (Λ f)·g ⇔ f[0:=g] case
+theorem β_induction_on (p: utlc → Prop): Π (f: utlc)
+  (down: Π n, p ↓n)
+  (lambda: Π x (hx: p x), p (Λ x))
+  (dot : Π x y (hx: p x) (hnx: ¬ ∃ x', Λ x' = x) (hy: p y), p (x·y))
+  (lambda_dot: Π x y (hx: p (Λ x)) (hx': p x) (hy: p y), p ((Λ x)·y)),
+  (p f)
+| (↓n) := λ hn hx hdx hlx, hn n
+| (Λ x) := λ hn hx hdx hlx, hx x (β_induction_on x hn hx hdx hlx)
+| (↓n·y) := λ hn hx hdx hlx, hdx (↓n) y (hn n) (by simp) (β_induction_on y hn hx hdx hlx)
+| ((Λ x)·y) := λ hn hx hdx hlx, hlx x y (β_induction_on (Λ x) hn hx hdx hlx) (β_induction_on x hn hx hdx hlx) (β_induction_on y hn hx hdx hlx)
+| (x·x'·y) := λ hn hx hdx hlx, hdx (x·x') y (β_induction_on (x·x') hn hx hdx hlx) (by simp) (β_induction_on y hn hx hdx hlx)
 
 end β
 end utlc
