src/lambda_calculus/utlc/reduction.lean
@@ -1,9 +1,8 @@
 import lambda_calculus.utlc.basic
+import lambda_calculus.utlc.identities
 
 namespace lambda_calculus
 namespace utlc
-
-local notation a `[` b `:=` c  `]` : 70 := has_substitution.substitution a b c
 
 def reduction_step : utlc → utlc → (utlc → utlc → Prop) → Prop
 | (↓ n) := λ g r, r (↓ n) g
@@ -16,43 +15,407 @@ def reduction_step : utlc → utlc → (utlc → utlc → Prop) → Prop
   | (↓_) := false
   | (Λ _) := false
   | (g1 · g2) :=
-    ((reduction_step f1 g1 r) ∧ f2 = g2) ∨ (f1 = g1 ∧ (reduction_step f2 g2 r))
+    (g2 = f2 ∧ (reduction_step f1 g1 r)) ∨ (g1 = f1 ∧ (reduction_step f2 g2 r))
   end
 
-theorem reduction_step_irrefl {head_step : utlc → utlc → Prop} :
-  (∀ f, ¬ head_step f f) → (∀ f, ¬ reduction_step f f head_step) :=
-begin
-  intros pf f,
-  induction f with _ f fh f g fh gh,
-  all_goals { simp[reduction_step, pf] },
-  exact fh,
-  exact not_or fh gh,
-end
-
-@[simp]
 def reduction_step_of := λ r f g, reduction_step f g r
 
-theorem reduction_step_lambda {f f' : utlc} {head_step : utlc → utlc → Prop}:
-  reduction_step f f' head_step → reduction_step (Λ f) (Λ f') head_step := or.inr
+section
+variables (head_step: utlc → utlc → Prop)
+variables (n : ℕ)
+variables (f f' g g': utlc)
+variables (m : ℕ)
 
-theorem application_reduction_step_left {f f' g : utlc} {head_step : utlc → utlc → Prop}:
-  reduction_step f f' head_step → reduction_step (f·g) (f'·g) head_step :=
+local attribute [simp] reduction_step reduction_step_of
+
+instance reduction_step.decidable_rel [h: decidable_rel head_step]: decidable_rel (reduction_step_of head_step) :=
 begin
-  intro n,
-  exact or.inr (or.inl ⟨n, rfl⟩)
+  have dor : ∀ (p q : Prop), decidable p → decidable q → decidable (p ∨ q),
+  { intros p q hp hq,
+    cases hp;
+    cases hq;
+    simp [hp, hq];
+    apply_instance },
+  have dand : ∀ (p q : Prop), decidable p → decidable q → decidable (p ∧ q),
+  { intros p q hp hq,
+    cases hp;
+    cases hq;
+    simp [hp, hq];
+    apply_instance },
+  intro f,
+  induction f;
+  intro g;
+  cases g;
+  simp;
+  repeat { apply dor };
+  repeat { apply dand };
+  try { apply_instance },
+  apply f_ih g,
+  apply f_ih_f g_f,
+  apply f_ih_g g_g
 end
 
-theorem application_reduction_step_right {f g g': utlc} {head_step : utlc → utlc → Prop}:
-  reduction_step g g' head_step → reduction_step (f·g) (f·g') head_step :=
+theorem down_reduction_step_iff: reduction_step_of head_step (↓n) g ↔ head_step (↓n) g :=
+by cases g; simp
+
+theorem lambda_reduction_step_iff: reduction_step_of head_step (Λ f) g ↔
+  head_step (Λ f) g ∨ ∃ x, g = Λ x ∧ reduction_step_of head_step f x :=
+by cases g; simp
+
+theorem dot_reduction_step_iff: reduction_step_of head_step (f·f') g ↔
+  head_step (f·f') g ∨
+    (∃ x, g = x·f' ∧ reduction_step_of head_step f x) ∨
+    ∃ x, g = f·x ∧ reduction_step_of head_step f' x :=
+by cases g; simp [and.assoc]
+end
+
+attribute [irreducible] reduction_step_of
+attribute [simp] down_reduction_step_iff lambda_reduction_step_iff dot_reduction_step_iff
+
+variables {head_step: utlc → utlc → Prop}
+variables {f f': utlc}
+variables {n: ℕ}
+variables {g g': utlc}
+variables {m: ℕ}
+
+@[simp] theorem reduction_step_down_iff:
+  reduction_step_of head_step f ↓m ↔ head_step f ↓m :=
+by cases f; simp
+
+theorem down_of_refl_trans_reduction_step:
+  (∀ n g, ¬ head_step (↓n:utlc) g) →
+  relation.refl_trans_gen (reduction_step_of head_step) (↓n:utlc) g →
+  g = ↓n :=
 begin
+  intros h p,
+  induction p with x g hfx hxg,
+  { refl },
+  rw [p_ih, down_reduction_step_iff] at hxg,
+  exfalso,
+  apply h _ _ hxg,
+end
+
+theorem reduction_step_lambda_iff:
+  reduction_step_of head_step f Λ g ↔
+  head_step f (Λ g) ∨ ∃ x, f = Λ x ∧ reduction_step_of head_step x g :=
+by cases f ; simp
+
+theorem reduction_step_dot_iff:
+  reduction_step_of head_step f (g·g') ↔
+  head_step f (g·g') ∨
+    (∃ x, x·g' = f ∧ reduction_step_of head_step x g) ∨
+    ∃ x, g·x = f ∧ reduction_step_of head_step x g' :=
+by cases f; simp [and.assoc]
+
+theorem lambda_reduction_step_lambda:
+  reduction_step_of head_step f g → reduction_step_of head_step (Λ f) (Λ g) :=
+by simp; exact or.inr
+
+theorem lambda_refl_reduction_step_lambda:
+  relation.refl_gen (reduction_step_of head_step) f g →
+  relation.refl_gen (reduction_step_of head_step) Λ f Λ g :=
+begin
+  intro p,
+  cases p,
+  { refl },
+  exact relation.refl_gen.single (lambda_reduction_step_lambda (by assumption)),
+end
+
+theorem lambda_refl_trans_reduction_step_lambda:
+  relation.refl_trans_gen (reduction_step_of head_step) f g →
+  relation.refl_trans_gen (reduction_step_of head_step) Λ f Λ g :=
+relation.refl_trans_gen.lift _ (@lambda_reduction_step_lambda _)
+
+theorem lambda_of_refl_trans_reduction_step:
+  (∀ f g, ¬ head_step (Λ f) g) →
+  relation.refl_trans_gen (reduction_step_of head_step) (Λ f) g →
+  ∃ x, g = Λ x :=
+begin
+  intros h p,
+  induction p with x g hfx hxg,
+  { use f },
+  cases p_ih with y hy,
+  rw [hy, lambda_reduction_step_iff] at hxg,
+  cases hxg,
+  { exfalso, apply h _ _ hxg },
+  rcases hxg with ⟨z, _, _⟩,
+  use z,
+  assumption,
+end
+
+theorem dot_reduction_step_dot_left:
+  reduction_step_of head_step f f' → reduction_step_of head_step (f·g) (f'·g) :=
+by intro p; simp [p]
+
+theorem dot_reduction_step_dot_right:
+  reduction_step_of head_step g g' → reduction_step_of head_step (f·g) (f·g') :=
+by intro p; simp [p]
+
+theorem dot_refl_reduction_step_dot_left:
+  relation.refl_gen (reduction_step_of head_step) f f' →
+  ∀ g, relation.refl_gen (reduction_step_of head_step) (f·g) (f'·g) :=
+begin
+  intros p _,
+  cases p,
+  { refl },
+  exact relation.refl_gen.single (dot_reduction_step_dot_left (by assumption))
+end
+
+theorem dot_refl_reduction_step_dot_right:
+  relation.refl_gen (reduction_step_of head_step) f f' →
+  ∀ g, relation.refl_gen (reduction_step_of head_step) (g·f) (g·f') :=
+begin
+  intros p _,
+  cases p,
+  { refl },
+  exact relation.refl_gen.single (dot_reduction_step_dot_right (by assumption))
+end
+
+theorem dot_refl_trans_reduction_step_dot_left:
+  relation.refl_trans_gen (reduction_step_of head_step) f f' →
+  ∀ g, relation.refl_trans_gen (reduction_step_of head_step) (f·g) (f'·g) :=
+begin
+  intros _ g,
+  simp only [show ∀ f, f·g = (λ x, x·g) f, by simp],
+  apply relation.refl_trans_gen.lift,
+  intros _ _ _,
+  apply dot_reduction_step_dot_left,
+  assumption'
+end
+
+theorem dot_refl_trans_reduction_step_dot_right:
+  relation.refl_trans_gen (reduction_step_of head_step) f f' →
+  ∀ g, relation.refl_trans_gen (reduction_step_of head_step) (g·f) (g·f') :=
+begin
+  intros _ g,
+  simp only [show ∀ f, g·f = (λ x, g·x) f, by simp],
+  apply relation.refl_trans_gen.lift,
+  intros _ _ _,
+  apply dot_reduction_step_dot_right,
+  assumption'
+end
+
+theorem dot_refl_trans_reduction_step_dot:
+  relation.refl_trans_gen (reduction_step_of head_step) f f' →
+  relation.refl_trans_gen (reduction_step_of head_step) g g' →
+  relation.refl_trans_gen (reduction_step_of head_step) (f·g) (f'·g') :=
+begin
+  intros p q,
+  apply trans,
+  exact dot_refl_trans_reduction_step_dot_left p _,
+  exact dot_refl_trans_reduction_step_dot_right q _
+end
+
+theorem  dot_of_refl_trans_reduction_step:
+  (∀ f f' g, ¬ head_step (f·f') g) →
+  relation.refl_trans_gen (reduction_step_of head_step) (f·f') g →
+  ∃ x x', g = x·x' :=
+begin
+  intros h p,
+  induction p with x g hfx hxg,
+  { exact ⟨f, f', rfl⟩ },
+  rcases p_ih with ⟨y, y', hy⟩,
+  rw [hy, dot_reduction_step_iff] at hxg,
+  obtain hxg|hxg|hxg := hxg;
+  try { exfalso, apply h _ _ _ hxg };
+  rcases hxg with ⟨z, hg, _⟩,
+  exact ⟨z, y', hg⟩,
+  exact ⟨y, z, hg⟩
+end
+
+theorem uses_zero_reduction_step  (h: ∀ {f g}, head_step f g → ∀ {n}, f.uses n = 0 → g.uses n = 0):
+  (reduction_step_of head_step f g) → ∀ {n}, f.uses n = 0 → g.uses n = 0 :=
+begin
+  induction f generalizing g;
+  simp only [down_notation, lambda_notation, dot_notation];
+  intro p;
+  try { rw [down_reduction_step_iff] at p };
+  try { rw [lambda_reduction_step_iff] at p, obtain p|p := p };
+  try { rw [dot_reduction_step_iff] at p, obtain p|p|p := p };
+  try { { apply @h _ _ p } };
+  rcases p with ⟨x, hg, hf⟩;
+  simp [hg];
   intro n,
-  exact or.inr (or.inr ⟨rfl, n⟩)
+  { apply f_ih hf },
+  { intros p q, exact ⟨ f_ih_f hf p, q ⟩ },
+  { intros p q, exact ⟨ p, f_ih_g hf q ⟩ }
+end
+
+theorem uses_reduction_step_uses (h: ∀ {f} {g}, head_step f g → ∀ n, f.uses n = g.uses n):
+  (reduction_step_of head_step f g) → ∀ n, f.uses n = g.uses n :=
+begin
+  induction f generalizing g;
+  simp only [down_notation, lambda_notation, dot_notation];
+  intro p;
+  try { rw [down_reduction_step_iff] at p };
+  try { rw [lambda_reduction_step_iff] at p, obtain p|p := p };
+  try { rw [dot_reduction_step_iff] at p, obtain p|p|p := p };
+  try { { apply h p } };
+  rcases p with ⟨x, hg, hf⟩;
+  simp [hg],
+  { intro n, apply f_ih hf },
+  { apply f_ih_f hf },
+  { apply f_ih_g hf }
+end
+
+theorem uses_refl_trans_reduction_step_uses (h: ∀ {f g}, head_step f g → ∀ n, f.uses n = g.uses n):
+  (relation.refl_trans_gen (reduction_step_of head_step) f g) → ∀ n, f.uses n = g.uses n :=
+begin
+  intro p,
+  induction p with x g hfx hxg,
+  { intro, refl },
+  intro n,
+  apply trans (p_ih _),
+  apply uses_reduction_step_uses @h hxg,
+end
+
+theorem shift_reduction_step_shift_iff: (∀ f g n, head_step (f ↑¹ n) (g ↑¹ n) ↔ head_step f g) → 
+  (reduction_step_of head_step (f ↑¹ n) (g ↑¹ n) ↔ reduction_step_of head_step f g) :=
+begin
+  intro p,
+  induction f generalizing n g;
+  simp;
+  conv_rhs { rw [← p _ _ n] };
+  simp,
+  { apply or_congr,
+    { refl },
+    split;
+    intro p,
+    { cases p with x p,
+      cases @shift_of_uses x (n+1) (by rw [← lambda_uses, ←p.left]; simp [shift_uses]) with y q,
+      use y,
+      rw [q] at p,
+      rw [← shift_inj_iff n, ← @f_ih (n + 1)],
+      simp [p] },
+    { cases p with x p,
+      use x ↑¹ (n + 1),
+      simp [p, f_ih] } },
+  { apply or_congr,
+    refl,
+    apply or_congr;
+    split;
+    intro p;
+    cases p with x p;
+    try { { use x ↑¹ n, simp [p, f_ih_f, f_ih_g] } },
+    { cases @shift_of_uses x n begin
+        conv_lhs { rw [← add_zero (x.uses n), ← shift_uses_zero' f_g n, ← dot_uses, ←p.left] };
+        apply shift_uses_zero'
+      end with y q,
+      use y,
+      rw [← shift_inj_iff n, ← @f_ih_f n],
+      simp [← q, p] },
+    { cases @shift_of_uses x n begin
+        conv_lhs { rw [← zero_add (x.uses n), ← shift_uses_zero' f_f n, ← dot_uses, ←p.left] };
+        apply shift_uses_zero'
+      end with y q,
+      use y,
+      rw [← shift_inj_iff n, ← @f_ih_g n],
+      simp [← q, p] } },
+end
+
+theorem shift_refl_trans_reduction_shift: (∀ f g n, head_step (f ↑¹ n) (g ↑¹ n) ↔ head_step f g) → 
+  (relation.refl_trans_gen (reduction_step_of head_step) f g → relation.refl_trans_gen (reduction_step_of head_step) (f ↑¹ n) (g ↑¹ n)) :=
+begin
+ intro p,
+ apply relation.refl_trans_gen.lift,
+ intros a b,
+ apply (shift_reduction_step_shift_iff p).mpr
+end
+
+local notation a `[` b `:=` c  `]` : 70 := has_substitution.substitution a b c
+
+theorem substitution_reduction_step_left (f: utlc) (hf: ∀ {f f'}, head_step f f' → ∀ n g, relation.refl_trans_gen (reduction_step_of head_step) (f[n:=g]) (f'[n:=g])): reduction_step_of head_step f f' →
+  ∀ n g, relation.refl_trans_gen (reduction_step_of head_step) (f[n:=g]) (f'[n:=g]) :=
+begin
+  induction f generalizing f';
+  simp;
+  intros p n g,
+  { apply hf p },
+  { cases p,
+    { apply hf p },
+    rcases p with ⟨x, hfx', hfx⟩,
+    rw [hfx'],
+    exact lambda_refl_trans_reduction_step_lambda (f_ih hfx _ _) },
+  { obtain p|p|p := p,
+    { apply hf p },
+    { rcases p with ⟨x, hfx', hfx⟩,
+      rw [hfx'],
+      exact dot_refl_trans_reduction_step_dot_left (f_ih_f hfx _ _) _ },
+    { rcases p with ⟨x, hfx', hfx⟩,
+      rw [hfx'],
+      exact dot_refl_trans_reduction_step_dot_right (f_ih_g hfx _ _) _ } }
+end
+
+theorem substitution_reduction_step_right (f: utlc) (hf: ∀ f g n, head_step (f ↑¹ n) (g ↑¹ n) ↔ head_step f g): reduction_step_of head_step g g' →
+  ∀ n, relation.refl_trans_gen (reduction_step_of head_step) (f[n:=g]) (f[n:=g']) :=
+begin
+  induction f generalizing g g';
+  simp;
+  intros p n,
+  { split_ifs,
+    refl,
+    apply relation.refl_trans_gen.single,
+    apply p,
+    refl },
+  { apply lambda_refl_trans_reduction_step_lambda,
+    apply f_ih,
+    rw shift_reduction_step_shift_iff,
+    assumption,
+    assumption },
+  { apply dot_refl_trans_reduction_step_dot,
+    apply f_ih_f,
+    assumption,
+    apply f_ih_g,
+    assumption }
 end
 
 def reduced : utlc → (utlc → bool) → bool
 | (↓ n) := λ p, p (↓ n)
 | (Λ f) := λ p, p (Λ f) ∧ reduced f p
 | (f · g) := λ p, p (f · g) ∧ reduced f p ∧ reduced g p
+
+def reduced_of : (utlc → bool) → utlc → bool := λ h f, reduced f h
+
+section
+local attribute [simp] reduced reduced_of
+variables (head_pred: utlc → bool)
+
+theorem down_reduced: reduced_of head_pred ↓n ↔ head_pred ↓n :=
+by simp
+
+theorem lambda_reduced: reduced_of head_pred Λ f ↔ head_pred Λ f ∧ reduced_of head_pred f :=
+by simp
+
+theorem dot_reduced: reduced_of head_pred (f·g) ↔ head_pred (f·g) ∧ reduced_of head_pred f ∧ reduced_of head_pred g :=
+by simp
+end
+attribute [irreducible] reduced_of
+attribute [simp] down_reduced lambda_reduced dot_reduced
+
+variables {head_pred: utlc → bool}
+
+theorem head_reduced_of_reduced: reduced_of head_pred f → head_pred f :=
+by { cases f; simp; repeat {intro }; assumption}
+
+theorem reduced_iff_not_reduction_step: (∀ f, head_pred f ↔ ∀ g, ¬ head_step f g) → (∀ f, reduced_of head_pred f ↔ ∀ g, ¬ reduction_step_of head_step f g) :=
+begin
+  intros p f,
+  induction f;
+  simp [p];
+  try { simp [f_ih] };
+  try { simp [f_ih_f, f_ih_g] };
+  split;
+  try { { intros q g, simp [q] } };
+  intro q;
+  split;
+  try { split };
+  intros g s;
+  try {
+  { apply q g, simp [s] } },
+  { apply q (Λ g), simp [s] },
+  { apply q (g·f_g), simp [s] },
+  { apply q (f_f·g), simp [s] }
+end
 
 end utlc
 end lambda_calculus
