src/complexity/basic.lean
@@ -1,0 +1,168 @@
+import tactic.basic
+
+lemma ftype {α α': Type} {β β': Type}: α = α' → β = β' → (α → β) = (α' → β') :=
+by { intros p q, rw [p, q] }
+
+lemma ftype_right (α: Type) {β β': Type}: β = β' → (α → β) = (α → β') :=
+by { intro p, rw [p] }
+
+lemma fcast: ∀ {α β γ: Type} (f: α → β) (a: α) (h: (β = γ)), (cast h (f a)) = (cast (ftype_right α h) f) a :=
+ by { intros α β γ f a h, finish }
+
+ lemma fcast': ∀ {α β γ: Type} (f: α → β) (a: α) (h: (β = γ)) (h': ((α → β) = (α → γ))), (cast h (f a)) = (cast h' f) a :=
+ by { intros α β γ f a h, finish }
+
+namespace complexity
+
+-- a model is a relation between a program type and a datatype
+structure model (α β γ: Type) [has_equiv β]  [preorder γ]  [has_add γ] :=
+mk ::
+  (accepts_with_cost : α → β → γ → Prop)
+  (application : α → β → α)
+  (cost_mono : ∀ {a : α} {b : β} {c₀ c₁ : γ}, c₀ ≤ c₁ → accepts_with_cost a b c₀ → accepts_with_cost a b c₁)
+
+variables {α β γ: Type} [has_equiv β] [preorder γ] [has_add γ]
+
+namespace model
+@[simp] def program_type: model α β γ → Type := λ _, α
+@[simp] def data_type: model α β γ → Type := λ _, β
+@[simp] def cost_type: model α β γ → Type := λ _, γ
+end model
+
+structure encoding (m: model α β γ) (δ: Type) :=
+mk ::
+  (encode: δ → β)
+  (encode_inj: ∀ x y: δ, encode x ≈ encode y ↔ x = y)
+
+variables {m: model α β γ}
+
+namespace encoding
+variables {δ: Type}
+
+@[simp] def model : encoding m δ → model α β γ := λ _,  m
+@[simp] def type : encoding m δ → Type := λ _, δ
+
+@[simp] def application (en: encoding m δ) (prog: α) (arg: δ): α :=
+  en.model.application prog (en.encode arg)
+
+@[simp] theorem inj_iff (en: encoding m δ) (a b: δ):
+  en.encode a ≈ en.encode b ↔ a = b := en.encode_inj _ _
+end encoding
+
+class has_encoding (m: model α β γ) (δ: Type):= (value: encoding m δ)
+
+def encode (m: model α β γ) {δ: Type} [f: has_encoding m δ] := f.value.encode
+
+inductive encodable_function (m: model α β γ): Type 1
+| result: Π {δ: Type}, encoding m δ → encodable_function
+| application: Π {δ: Type}, encoding m δ → encodable_function → encodable_function
+
+namespace encodable_function
+@[simp] def model : encodable_function m → model α β γ := λ _, m
+
+@[simp] def unwrap: encodable_function m → Type
+| (result en) := en.type
+| (application en b) := en.type → b.unwrap
+end encodable_function
+variables {enf: encodable_function m}
+
+structure is_encoded_function (m: model α β γ) (δ: Type):=
+mk ::
+  (value: encodable_function m)
+  (sound: value.unwrap = δ)
+
+class has_encodable_function (m: model α β γ) (δ: Type) := (value: is_encoded_function m δ)
+
+variables {δ: Type} [has_encodable_function m δ]
+
+@[simp] theorem unwrap_has_encodable (a: has_encodable_function m δ): a.value.value.unwrap = δ := a.value.sound
+theorem unwrap_has_encodable' (a: has_encodable_function m δ): δ = a.value.value.unwrap := a.value.sound.symm
+
+@[simp] theorem unwrap_is_encoded_function (a: is_encoded_function m δ): a.value.unwrap = δ := a.sound
+
+def cast_unwrap [a: has_encodable_function m δ] (f: δ): a.value.value.unwrap :=
+  cast (unwrap_has_encodable' a) f
+
+instance encodable_result (δ: Type) [f: has_encoding m δ]:
+    has_encodable_function m δ :=
+  ⟨ ⟨ encodable_function.result f.value, rfl ⟩ ⟩
+
+instance encodable_application (δ: Type) [f: has_encoding m δ] (ε: Type) [g: has_encodable_function m ε]:
+    has_encodable_function m (δ → ε) :=
+  ⟨ ⟨ encodable_function.application f.value g.value.value, ftype rfl g.value.sound ⟩ ⟩
+
+def cost_function: encodable_function m → Type
+| (encodable_function.result _) := γ
+| (encodable_function.application en c) := en.type → cost_function c
+
+@[simp] def cost_function' (m: model α β γ) (δ : Type) [f: has_encodable_function m δ] := cost_function f.value.value
+
+namespace cost_function
+variables {cf₀ cf₁ : cost_function enf}
+
+def less_than_or_equal: Π {enf: encodable_function m}, cost_function enf → cost_function enf → Prop
+| (encodable_function.result _) := λ n m: γ, n ≤ m
+| (encodable_function.application _ _) := λ f g, ∀ a, less_than_or_equal (f a) (g a)
+
+instance: preorder (cost_function enf) := begin
+  fconstructor,
+  exact cost_function.less_than_or_equal,
+  induction enf,
+  { intro cf, refl },
+  { intros cf x, exact enf_ih _ },
+  induction enf,
+  { intros a b c,
+    apply preorder.le_trans},
+  { intros a b c hab hac x,
+    exact enf_ih _ _ _ (hab x) (hac x) },
+end
+
+def add: Π {enf: encodable_function m}, cost_function enf → cost_function enf → cost_function enf
+| (encodable_function.result _) := λ n m: γ, (n + m: γ)
+| (encodable_function.application _ _) := λ f g a, add (f a) (g a)
+
+instance: has_add (cost_function enf) := ⟨ add ⟩
+
+def lift: Π (enf: encodable_function m), γ → cost_function enf
+| (encodable_function.result _) := λ c, c
+| (encodable_function.application _ enf) := λ c _, lift enf c
+
+instance: has_lift γ (cost_function enf) := ⟨ lift enf ⟩
+
+end cost_function
+
+def witness: Π (a : encodable_function m), α → a.unwrap → (cost_function a) → Prop
+| (encodable_function.result en) := λ prog data, en.model.1 prog (en.encode data)
+| (encodable_function.application en b) := λ prog f cost, ∀ arg : en.type,
+  witness b (encoding.application en prog arg) (f arg) (cost arg)
+
+def complexity_le [enf: has_encodable_function m δ] (f: δ) (cf: cost_function enf.value.value) :=
+  ∃ prog: α, witness enf.value.value prog (cast_unwrap f) cf
+
+structure is_complexity (m: model α β γ) {δ: Type} [has_encodable_function m δ] (f: δ) :=
+mk ::
+  (cost : cost_function' m δ)
+  (proof : complexity_le f cost)
+
+class has_complexity (m: model α β γ) {δ: Type} [has_encodable_function m δ] (f: δ) :=
+  (value: is_complexity m f)
+
+theorem omega_equiv  {m: model α β γ} {δ: Type} [enf: has_encodable_function m δ] {f: δ} {cf: cost_function enf.value.value}:
+  complexity_le f cf → ∀ g, f = g → complexity_le g cf :=
+begin
+  intros hf g hfg,
+  rw [← hfg],
+  exact hf,
+end
+
+end complexity
+
+def complexity {α β γ: Type} [has_equiv β] [preorder γ] [has_add γ]
+  (m: complexity.model α β γ) {δ: Type} [complexity.has_encodable_function m δ]
+  (f: δ) [c: complexity.has_complexity m f]:
+  complexity.cost_function' m δ := c.value.cost
+
+instance {α β γ: Type} [has_equiv β] [preorder γ] [has_add γ] (m: complexity.model α β γ)
+  (δ: Type) [complexity.has_encodable_function m δ]:
+  has_le (complexity.cost_function' m δ) :=
+  ⟨ complexity.cost_function.less_than_or_equal ⟩
