src/complexity/nat.lean
@@ -1,0 +1,35 @@
+import complexity.basic
+import complexity.core
+import tactic.linarith
+
+
+namespace complexity
+namespace nat
+
+variables {mα mβ mγ: Type} [has_equiv mβ] [preorder mγ] [has_add mγ]
+variables {m: model mα mβ mγ}
+
+instance mul_complexity [has_encoding m ℕ] [has_encoding m (ℕ×ℕ)]
+  [cf: has_complexity m
+    (curry (compose
+      prod.fst
+      ((compose
+        (uncurry (nat.iterate (fork (uncurry nat.add) prod.snd)))
+        (((fork prod.snd (fork (@const ℕ (ℕ×ℕ) 0) prod.fst))))))))]:
+  has_complexity m nat.mul :=
+begin
+  fconstructor,
+  fconstructor,
+  exact cf.value.cost,
+  apply omega_equiv cf.value.proof,
+  clear cf,
+  ext1 n, ext1 m,
+  apply (show ∀ (c: ℕ) (a: ℕ×ℕ) (b: ℕ), a = (b, c) → a.fst = b, by finish) n,
+  simp [compose, flip, fork, to_fst, function.uncurry, const, curry, uncurry],
+  induction m,
+  { simp, },
+  simp [function.iterate_succ', nat.mul_succ, m_ih],
+end
+
+end nat
+end complexity
