src/lambda_calculus/utlc/beta/complexity/basic.lean
@@ -1,0 +1,140 @@
+import lambda_calculus.utlc.beta.distance
+import lambda_calculus.utlc.beta.encoding.basic
+import complexity.basic
+import complexity.core
+
+namespace lambda_calculus
+namespace utlc
+namespace β
+namespace complexity
+
+open lambda_calculus.utlc.β.encoding
+
+local attribute [simp] closed closed_below
+local attribute [simp] β.normal_iteration β.strategic_reduction_step
+local attribute [simp] reduced substitution shift shift_substitution_index
+
+theorem of_distance_le
+  {a: complexity.encodable_function distance_model} {f f': a.unwrap} (g : encoded_program) {g': encoded_program} (fc fc': complexity.cost_function a) (n: ℕ):
+  distance_le n g'.value g.value → complexity.witness a g f fc → f = f' → (fc + ↑n) ≤ fc' →
+  complexity.witness a g' f' fc' :=
+begin
+  induction a with _ _ _ en _ generalizing f f' g g' fc fc',
+  { intros hg hw hf hfc,
+    rw [← hf],
+    apply distance_le_mono,
+    apply distance_le_trans',
+    apply hg,
+    apply hw,
+    refl,
+    rw  [nat.cast_id, nat.add_comm] at hfc,
+    assumption },
+  { intros hg hw hf hfc a,
+    apply a_ih (en.application g a),
+    simp [distance_model],
+    apply utlc.β.dot_distance_le_dot_left,
+    apply hg,
+    apply hw,
+    rw [hf],
+    apply hfc,
+  }
+end
+
+instance value_complexity (α: Type) [en: complexity.has_encoding distance_model α] (a: α):
+  complexity.has_complexity distance_model a :=
+  ⟨ ⟨ (0:ℕ),
+    ⟨ ⟨ (en.value.encode a).value, (en.value.encode a).proof.left ⟩,
+      @distance_le_refl _ has_β_reduction.step _ ⟩ ⟩ ⟩
+
+def id_prog: encoded_program := ⟨ Λ ↓0, by simp ⟩
+
+instance id_complexity (α: Type) [en: complexity.has_encoding distance_model α] (a: α):
+  complexity.has_complexity distance_model (@id α) :=
+  ⟨ ⟨ λ _, (1:ℕ), ⟨ id_prog,
+begin
+  intro a,
+  apply distance_le_of_normal_iteration,
+  simp [id_prog, complexity.cast_unwrap, distance_model],
+end ⟩ ⟩ ⟩
+
+def const_prog: encoded_program := ⟨ Λ Λ ↓1, by simp ⟩
+
+instance const_complexity (α β: Type) [en: complexity.has_encoding distance_model α] [en: complexity.has_encoding distance_model β]:
+  complexity.has_complexity distance_model (@const α β) :=
+  ⟨ ⟨ λ _ _, (2:ℕ), ⟨ const_prog,
+begin
+  intros a b,
+  apply distance_le_of_normal_iteration,
+  simp [const_prog, const, complexity.cast_unwrap, distance_model],
+end ⟩ ⟩ ⟩
+
+instance partial_complexity
+  (α β: Type) [en: complexity.has_encoding distance_model α]  [complexity.has_encodable_function distance_model β]
+  (a: α) {f: α → β} [h: complexity.has_complexity distance_model f] :
+  complexity.has_complexity distance_model (f a) :=
+  ⟨ ⟨ (complexity distance_model f) a,
+  by {
+  cases h.value.proof with prog h,
+  exact ⟨ ⟨ prog.value·(en.value.encode a).value, by {
+    simp only [ bool.to_bool_coe, and_true,
+      data_is_closed_below', closed_below, closed], apply prog.proof } ⟩,
+  by { rw [complexity.cast_unwrap, fcast], exact h a } ⟩ } ⟩ ⟩
+
+def compose_prog: encoded_program := ⟨ Λ Λ Λ ↓2·(↓1·↓0), by simp ⟩
+
+instance compose_complexity
+  (α β γ: Type) [α_en: complexity.has_encoding distance_model α] [β_en: complexity.has_encoding distance_model β] [γ_en: complexity.has_encodable_function distance_model γ]
+  (f: α → β) (g: β → γ) [cf: complexity.has_complexity distance_model f] [cg: complexity.has_complexity distance_model g] : complexity.has_complexity distance_model (compose g f) :=
+⟨ ⟨ λ a, cg.value.cost (f a) + ↑(3 + (cf.value.cost a):ℕ),
+begin
+  rcases cf.value with ⟨cfc, fp, cfp⟩,
+  rcases cg.value with ⟨cgc, gp, cgp⟩,
+  fconstructor,
+  { exact ⟨ compose_prog.value·gp.value·fp.value,
+    by simp; exact ⟨compose_prog.proof, gp.proof, fp.proof⟩ ⟩ },
+  intro a,
+  apply of_distance_le begin
+    fconstructor,
+    { exact gp.value·((β_en.value.encode (f a)).value) },
+    simp, exact  gp.proof,
+  end,
+  { simp [distance_model, compose_prog],
+    apply distance_le_trans,
+    { apply distance_le_of_normal_iteration 3,
+      simp [normal_iteration, distance_model, compose_prog] },
+    rw [← shift_comm _ (nat.zero_le _)],
+    simp [shift_substitution_index],
+    apply utlc.β.dot_distance_le_dot_right,
+    apply cfp a },
+  apply cgp (f a),
+  unfold complexity.cast_unwrap,
+  rw [← fcast', ← fcast'],
+  all_goals { simp [compose] },
+end ⟩ ⟩
+
+def flip_prog: encoded_program := ⟨ Λ Λ Λ ↓2·↓0·↓1, by simp ⟩
+
+instance flip_complexity
+  (α β γ: Type) [α_en: complexity.has_encoding distance_model α] [β_en: complexity.has_encoding distance_model β] [γ_en: complexity.has_encoding distance_model γ]
+  (f: α → β → γ) [cf: complexity.has_complexity distance_model f]: complexity.has_complexity distance_model (flip f) :=
+⟨ ⟨ λ b a, (cf.value.cost a b) + ↑3,
+begin
+  rcases cf.value with ⟨cfc, fp, cfp⟩,
+  fconstructor,
+  { exact ⟨ flip_prog.value·fp.value,
+    by simp; exact ⟨ flip_prog.proof, fp.proof ⟩ ⟩ },
+  intros a b,
+  apply distance_le_trans',
+  { apply distance_le_of_normal_iteration 3,
+    refl },
+  simp [distance_model, flip_prog],
+  rw [← shift_comm _ (nat.zero_le _)],
+  simp [shift_substitution_index],
+  apply cfp,
+  simp [add_comm 3],
+end ⟩ ⟩
+
+end complexity
+end β
+end utlc
+end lambda_calculus
