src/lambda_calculus/utlc/beta/complexity/core.lean
@@ -1,0 +1,127 @@
+import lambda_calculus.utlc.beta.distance
+import lambda_calculus.utlc.beta.encoding.basic
+import lambda_calculus.utlc.beta.encoding.core
+import lambda_calculus.utlc.beta.complexity.basic
+import complexity.basic
+import complexity.core
+
+namespace lambda_calculus
+namespace utlc
+namespace β
+namespace complexity
+
+open complexity
+open lambda_calculus.utlc.β.encoding
+
+local attribute [simp] closed closed_below
+local attribute [simp] β.normal_iteration β.strategic_reduction_step
+local attribute [simp] reduced substitution shift shift_substitution_index
+
+def fork_prog: encoded_program := ⟨ Λ Λ Λ Λ ↓0·(↓3·↓1)·(↓2·↓1), by simp [←one_add_one_eq_two] ⟩
+
+instance fork_complexity_le {α β γ: Type} [complexity.has_encoding distance_model α] [complexity.has_encoding distance_model β] [complexity.has_encoding distance_model γ]
+  {f: α → β} [cf: complexity.has_complexity distance_model f]
+  {g: α → γ} [cg: complexity.has_complexity distance_model g]:
+  complexity.has_complexity distance_model (fork f g) :=
+⟨ ⟨ (λ a, (3:ℕ) + (cf.value.cost a + cg.value.cost a)),
+begin
+  rcases cf.value with ⟨cfc, fp, cfp⟩,
+  rcases cg.value with ⟨cgc, gp, cgp⟩,
+  fconstructor,
+  fconstructor,
+  exact fork_prog.value·fp.value·gp.value,
+  simp,
+  exact ⟨ fork_prog.proof, fp.proof, gp.proof ⟩,
+  intro a,
+  apply distance_le_trans',
+  apply distance_le_of_normal_iteration 3,
+  simp [fork_prog, complexity.cast_unwrap, distance_model, ← shift_comm _ (nat.zero_le _),
+    complexity.has_encoding.value],
+  rw [shift_of_closed fp.proof, shift_of_closed gp.proof, shift_of_closed],
+  apply lambda_distance_le_lambda,
+  apply distance_le_trans',
+  apply dot_distance_le_dot_left,
+  apply dot_distance_le_dot_right,
+  apply cfp,
+  apply dot_distance_le_dot_right,
+  apply cgp,
+  refl,
+  simp,
+end
+⟩ ⟩
+
+def curry_prog: encoded_program := ⟨ Λ Λ Λ ↓2·(Λ ↓0·↓2·↓1), by simp[← one_add_one_eq_two] ⟩
+
+instance curry_complexity_le {α β γ: Type} [α_en: complexity.has_encoding distance_model α] [β_en: complexity.has_encoding distance_model β] [complexity.has_encodable_function distance_model γ]
+  {f: (α × β) → γ} [cf: complexity.has_complexity distance_model f]:
+  complexity.has_complexity distance_model (curry f) :=
+⟨ ⟨ (λ a b, (cf.value.cost (a, b) + ↑(3:ℕ))),
+begin
+  rcases cf.value with ⟨cfc, fp, cfp⟩,
+  fconstructor,
+  fconstructor,
+  exact curry_prog.value·fp.value,
+  simp,
+  exact ⟨ curry_prog.proof, fp.proof ⟩,
+  intros a b,
+  apply of_distance_le begin
+    fconstructor,
+    refine fp.value·_,
+    apply encoding.encoded_data.value,
+    apply complexity.encode distance_model,
+    apply (a, b),
+    apply @encoding.prod_encoding α β α_en β_en,
+    simp,
+    apply fp.proof,
+  end,
+  apply distance_le_of_normal_iteration 3,
+  simp [curry_prog, complexity.cast_unwrap, distance_model, complexity.has_encoding.value, ← shift_comm _ (nat.zero_le _)],
+  rw [shift_of_closed, shift_of_closed, complexity.encode],
+  refl,
+  simp,
+  simp,
+  apply cfp,
+  simp [complexity.cast_unwrap, ← fcast', curry],
+end
+⟩ ⟩
+
+def uncurry_prog: encoded_program := ⟨ Λ Λ ↓0·↓1, by simp ⟩
+
+instance uncurry_complexity_le {α β γ: Type} [α_en: complexity.has_encoding distance_model α] [β_en: complexity.has_encoding distance_model β] [complexity.has_encodable_function distance_model γ]
+  {f: α → β → γ} [cf: complexity.has_complexity distance_model f]:
+  complexity.has_complexity distance_model (uncurry f) :=
+⟨ ⟨ (λ ab, (cf.value.cost ab.fst ab.snd + ↑(3:ℕ))),
+begin
+  rcases cf.value with ⟨cfc, fp, cfp⟩,
+  fconstructor,
+  fconstructor,
+  exact uncurry_prog.value·fp.value,
+  simp,
+  exact ⟨ uncurry_prog.proof, fp.proof ⟩,
+  intros ab,
+  cases ab with a b,
+  apply of_distance_le begin
+    fconstructor,
+    refine fp.value·_·_,
+    apply encoding.encoded_data.value,
+    apply complexity.encode distance_model,
+    apply a,
+    apply α_en,
+    apply encoding.encoded_data.value,
+    apply complexity.encode distance_model,
+    apply b,
+    apply β_en,
+    simp,
+    apply fp.proof,
+  end,
+  apply distance_le_of_normal_iteration 3,
+  simp [uncurry_prog, pair, complexity.cast_unwrap, distance_model, complexity.has_encoding.value, ← shift_comm _ (nat.zero_le _), substitution_identity_of_closed],
+  simp [complexity.encode],
+  apply cfp,
+  simp [complexity.cast_unwrap, ← fcast', uncurry],
+end ⟩ ⟩
+
+end complexity
+end β
+end utlc
+end lambda_calculus
