src/lambda_calculus/utlc/beta/complexity/nat.lean
@@ -1,0 +1,143 @@
+import lambda_calculus.utlc.beta.distance
+import lambda_calculus.utlc.beta.encoding.basic
+import lambda_calculus.utlc.beta.encoding.core
+import lambda_calculus.utlc.beta.encoding.nat
+import lambda_calculus.utlc.beta.complexity.core
+import complexity.basic
+import complexity.nat
+
+open complexity
+open lambda_calculus.utlc.β.encoding
+
+namespace lambda_calculus
+namespace utlc
+namespace β
+namespace complexity
+namespace nat
+
+
+local attribute [simp] distance_model closed closed_below
+local attribute [simp] β.normal_iteration β.strategic_reduction_step
+local attribute [simp] reduced substitution shift shift_substitution_index
+
+def succ_prog: encoded_program := ⟨ Λ Λ Λ ↓1·(↓2·↓1·↓0), by simp ⟩
+
+instance succ_complexity: has_complexity distance_model nat.succ :=
+  ⟨ ⟨ λ _, (3:ℕ), ⟨ succ_prog,
+begin
+  simp only [cast_unwrap, cast_eq],
+  intros n,
+  apply β.distance_le_of_normal_iteration 3,
+  simp [succ_prog, has_encoding.value, encoding.nat.iterate, function.iterate_succ']
+end ⟩ ⟩ ⟩
+
+def add_prog: encoded_program := ⟨ Λ Λ Λ Λ ↓3·↓1·(↓2·↓1·↓0), by simp [← one_add_one_eq_two] ⟩
+
+instance add_complexity: has_complexity distance_model nat.add :=
+  ⟨ ⟨ λ _ _, (6:ℕ), ⟨ add_prog,
+begin
+  simp only [cast_unwrap, cast_eq],
+  intros n m,
+  apply distance_le_trans' 4 2,
+  apply β.distance_le_of_normal_iteration,
+  simp [add_prog, has_encoding.value, function.iterate_succ'],
+  apply β.lambda_distance_le_lambda,
+  apply β.lambda_distance_le_lambda,
+  induction n generalizing m,
+  { cases m;
+    apply β.distance_le_of_normal_iteration;
+    simp [function.iterate_succ', function.iterate_zero, encoding.nat.iterate] },
+  simp [function.iterate_succ', function.iterate_zero, encoding.nat.iterate, nat.succ_add],
+  apply β.dot_distance_le_dot_right,
+  apply n_ih,
+  simp,
+end ⟩ ⟩ ⟩  
+
+def iterate_prog: encoded_program := ⟨ Λ Λ Λ ↓1·↓2·↓0, by simp ⟩
+
+namespace iteration_complexity
+
+lemma iterate_distance_le {n: ℕ} {f g: utlc}: distance_le n f g → ∀ (a: utlc) (m: ℕ), distance_le n ((has_dot.dot a)^[m] f) ((has_dot.dot a)^[m] g) :=
+begin
+  intros hfg a m,
+  induction m generalizing f g,
+  simp [hfg],
+  simp,
+  apply m_ih,
+  apply dot_distance_le_dot_right hfg,
+end
+
+def cost {α: Type}
+  (fi: α → α) (ni: α → ℕ): ℕ → α → ℕ
+| 0 := λ fz, 5
+| (n+1) := λ fz, (ni fz) + (cost n (fi fz)) + 10
+
+theorem cost_zero {α: Type} (fi: α → α) (ni: α → ℕ) (a: α): cost fi ni 0 a = 5 := rfl
+
+theorem cost_succ {α: Type} (fi: α → α) (ni: α → ℕ) (n: ℕ) (a: α): cost fi ni (n + 1) a = (ni a) + cost fi ni n (fi a) + 10 := rfl
+
+theorem cost_succ' {α: Type} (fi: α → α) (ni: α → ℕ) (n: ℕ) (a: α): cost fi ni (n + 1) a = (ni (fi^[n] a)) + cost fi ni n a + 10 :=
+begin
+  rw [cost_succ],
+  induction n generalizing a,
+  simp [cost_zero],
+  rw [cost_succ, n_ih, cost_succ, function.iterate_succ],
+  simp [nat.add_assoc, nat.add_left_comm _ (ni a)],
+end
+
+@[simp] def cost' {α: Type} [α_en: has_encoding distance_model α]
+  (fi: α → α) (ni: complexity.cost_function' distance_model (α → ℕ)): complexity.cost_function' distance_model (ℕ → α → α) := cost fi ni
+end iteration_complexity
+
+instance iteration_complexity (α: Type) [α_en: has_encoding distance_model α]
+  (f: α → α) [cf: has_complexity distance_model f]: has_complexity distance_model (nat.iterate f) :=
+⟨ ⟨ iteration_complexity.cost' f cf.value.cost,
+begin
+  rcases cf.value with ⟨cfc, fp, cfp⟩,
+  fconstructor,
+  use iterate_prog.value·fp.value,
+  { simp, exact ⟨ iterate_prog.proof, fp.proof ⟩ },
+  simp only [cast_unwrap, cast_eq, iterate_prog],
+  intros n a,
+  induction n generalizing a,
+  { apply β.distance_le_of_normal_iteration,
+    simp [has_encoding.value, ← shift_comm _ (nat.zero_le _), shift_substitution_index, encoding.nat.iterate, iteration_complexity.cost_zero] },
+  { apply distance_le_trans',
+    apply β.distance_le_of_normal_iteration 5,
+    refl,
+    simp [has_encoding.value, ← shift_comm _ (nat.zero_le _), shift_substitution_index, encoding.nat.iterate],
+    apply distance_le_trans' (5 + (cfc a)) _ _ (n_ih (f a)),
+    all_goals { clear n_ih },
+    refl,
+    simp [has_encoding.value, encoding.nat.iterate],
+    apply distance_le_symm,
+    apply distance_le_trans',
+    apply β.distance_le_of_normal_iteration 5,
+    simp [← shift_comm _ (nat.zero_le _), shift_substitution_index],
+    apply distance_le_symm,
+    simp [encoding.nat.iterate],
+    apply iteration_complexity.iterate_distance_le,
+    apply cfp,
+    refl,
+    simp [iteration_complexity.cost_succ],
+    ring }
+end ⟩ ⟩
+
+example:  (complexity distance_model nat.mul) ≤ (λ (x y: ℕ), ((30*y + 43):ℕ)) :=
+begin
+  intros n m,
+  simp only [complexity, complexity.cost_function.less_than_or_equal, has_complexity.value, fork, const, uncurry],
+  ring_nf,
+  norm_num,
+  induction m,
+  { simp only [iteration_complexity.cost_zero],
+    ring_nf },
+  simp only [iteration_complexity.cost_succ', function.iterate_succ', nat.mul_succ, add_mul, nat.add_assoc],
+  nlinarith,
+end
+
+end nat
+end complexity
+end β
+end utlc
+end lambda_calculus
