src/lambda_calculus/utlc/beta/encoding/basic.lean
@@ -1,0 +1,53 @@
+import lambda_calculus.utlc.beta.distance
+import complexity.basic
+
+namespace lambda_calculus
+namespace utlc
+namespace β
+namespace encoding
+
+structure encoded_program :=
+mk :: (value: utlc) (proof: value.closed)
+
+structure encoded_data :=
+mk :: (value: utlc) (proof: value.closed ∧ β.reduced value)
+
+instance : has_equiv encoded_data := ⟨ λ a b : encoded_data, a.value = b.value ⟩
+
+local attribute [reducible] closed
+
+def distance_model : complexity.model encoded_program encoded_data ℕ :=
+ ⟨ λ prog data cost, distance_le cost prog.value data.value,
+   λ prog data, ⟨ prog.value·data.value, by simp [closed, prog.proof, data.proof.left] ⟩,
+   λ prog data c₀ c₁, distance_le_mono' ⟩
+
+  
+@[simp] theorem data_is_closed_below (a: encoded_data):
+  ∀ n, a.value.closed_below n :=
+  λ n, closed_below_mono a.proof.left (nat.zero_le _)
+
+@[simp] theorem data_is_closed_below' {α: Type}
+  [f: complexity.has_encoding distance_model α]
+  (a: α) : ∀ n, (f.value.encode a).value.closed_below n :=
+  λ n, closed_below_mono (f.value.encode a).proof.left (nat.zero_le _)
+
+@[simp] theorem data_is_reduced (a: encoded_data):
+   reduced_of head_reduced a.value := a.proof.right
+
+@[simp] theorem data_is_reduced' {α: Type}
+  [f: complexity.has_encoding distance_model α]
+  (a: α) : reduced_of head_reduced (f.value.encode a).value :=
+  (f.value.encode a).proof.right
+
+@[simp] theorem value_inj (a b: encoded_data):
+  a ≈ b ↔ a.value = b.value := by refl
+
+@[simp] theorem data_value_inj {α: Type}
+  [f: complexity.has_encoding distance_model α] (a b: α):
+  (f.value.encode a).value = (f.value.encode b).value ↔ a = b :=
+by rw [← value_inj, complexity.encoding.inj_iff]
+
+end encoding
+end β
+end utlc
+end lambda_calculus
