src/lambda_calculus/utlc/beta/encoding/core.lean
@@ -1,0 +1,80 @@
+import lambda_calculus.utlc.beta.distance
+import complexity.basic
+import lambda_calculus.utlc.beta.encoding.basic
+
+namespace lambda_calculus
+namespace utlc
+namespace β
+namespace encoding
+
+def false : utlc := Λ Λ ↓0
+def true : utlc := Λ Λ ↓1
+
+instance bool_encoding: complexity.has_encoding distance_model bool :=
+  ⟨ ⟨ λ b, ⟨ ite b true false,
+     by cases b; simp[true, false, closed_below] ⟩,
+     by intros x y; cases x; cases y; simp [false, true]  ⟩ ⟩
+
+instance decidable_encoding (p: Prop): complexity.has_encoding distance_model (decidable p) :=
+  ⟨ ⟨ λ dp, ⟨ @ite _ p dp true false,
+    by split_ifs; simp[true, false, closed] ⟩,
+    by finish ⟩ ⟩
+
+def pair (f g: encoded_data): encoded_data :=
+  ⟨ Λ ↓0·f.value·g.value, by simp ⟩
+
+instance prod_encoding {α β: Type*}
+  [f: complexity.has_encoding distance_model α]
+  [g: complexity.has_encoding distance_model β]:
+  complexity.has_encoding distance_model (α × β) :=
+  ⟨ ⟨ λ ab, pair (f.value.encode ab.fst) (g.value.encode ab.snd),
+      by intros x y; cases x; cases y; simp [pair, and_imp] ⟩ ⟩
+
+def alternative {n m: ℕ} (h: n < m) (f: encoded_data): encoded_data := ⟨
+  ( λ x, Λ x)^[m] (↓n·f.value),
+    begin
+      split,
+      { cases nat.exists_eq_add_of_le (nat.succ_le_of_lt h) with y h,
+        rw [h, add_comm, function.iterate_add_apply],
+        clear h h,
+        apply show ∀ y (f: utlc), f.closed → ((λ x :utlc, Λ x)^[y] f).closed,
+        begin
+          intro y,
+          induction y,
+          { simp },
+          intros f hf,
+          simp [function.iterate_succ', function.comp_app,
+            lambda_reduced_iff, closed, closed_below, add_zero,
+            closed_below_mono (y_ih f hf)],
+        end,
+        apply show ∀ n (f: utlc), f.closed_below n → ((λ x :utlc, Λ x)^[n] f).closed,
+        begin
+          intro n,
+          induction n,
+          { simp },
+          intros f hf,
+          simp only [function.iterate_succ, function.comp_app,
+            n_ih (Λ f) (by simp [hf])],
+        end,
+        simp [nat.lt_succ_self],
+      },
+      clear h,
+      induction m,
+      { simp },
+      simp only [function.iterate_succ', function.comp_app, lambda_reduced_iff, m_ih]
+    end ⟩
+
+namespace either
+@[simp] def left: encoded_data → encoded_data := alternative (show 0 < 2, by simp)
+@[simp] def right: encoded_data → encoded_data := alternative (show 1 < 2, by simp)
+end either
+
+instance sum_encoding {α β: Type*} [f: complexity.has_encoding distance_model α] [g: complexity.has_encoding distance_model β]:
+  complexity.has_encoding distance_model (α ⊕ β) := ⟨ ⟨ λ ab,
+    sum.elim (either.left ∘ f.value.encode) (either.right ∘ g.value.encode) ab,
+    by intros a b; cases a; cases b; simp [alternative] ⟩ ⟩
+
+end encoding
+end β
+end utlc
+end lambda_calculus
