src/lambda_calculus/utlc/beta/encoding/nat.lean
@@ -1,0 +1,66 @@
+import lambda_calculus.utlc.beta.distance
+import complexity.basic
+import lambda_calculus.utlc.beta.encoding.basic
+
+namespace lambda_calculus
+namespace utlc
+namespace β
+namespace encoding
+namespace nat
+
+@[reducible] def iterate (f: utlc) (n: ℕ) (g: utlc): utlc := (λ x, f·x)^[n] g
+
+section
+local notation a `[` b `:=` c  `]` : 70 := has_substitution.substitution a b c
+
+@[simp] theorem iterate_substitution {n m: ℕ} {f g x: utlc}:
+  (iterate f n g)[m:=x] = (iterate (f[m:=x]) n (g[m:=x])) :=
+begin
+  induction n;
+  simp[iterate, function.iterate_succ'],
+  apply n_ih
+end
+
+@[simp] theorem iterate_shift {n m: ℕ} {f g: utlc}:
+  (iterate f n g) ↑¹ m = (iterate (f ↑¹ m) n (g ↑¹ m)) :=
+begin
+  induction n,
+  all_goals { simp[iterate, function.iterate_succ'] },
+  apply n_ih
+end
+end
+
+instance nat_encoding:
+  complexity.has_encoding distance_model ℕ := ⟨ ⟨ λ n,
+    ⟨ (Λ Λ iterate (↓1:utlc) n ↓0: utlc),
+      begin
+        induction n,
+        { simp [iterate] },
+        simp only [iterate, reduced, lambda_reduced, closed, closed_below,
+          zero_add, one_add_one_eq_two] at n_ih,
+        simp [function.iterate_succ', iterate, n_ih],
+      end
+    ⟩,
+    begin
+      intros x y,
+      cases le_total x y;
+      cases nat.exists_eq_add_of_le h with z h;
+      rw [h];
+      clear h;
+      simp only [iterate, value_inj, lambda_eq_lambda_iff, self_eq_add_right];
+      cases z;
+      try { { simp } };
+      clear h,
+      { induction x,
+        { simp [function.iterate_succ'] },
+        simp [function.iterate_succ', nat.succ_add, x_ih] },
+      { induction y,
+        { simp [function.iterate_succ'] },
+        simp [function.iterate_succ', nat.succ_add, y_ih], }
+    end ⟩ ⟩
+
+end nat
+end encoding
+end β
+end utlc
+end lambda_calculus
