src/lambda_calculus/utlc/beta/encoding/utlc.lean
@@ -1,0 +1,32 @@
+import lambda_calculus.utlc.basic
+import lambda_calculus.utlc.beta.basic
+import lambda_calculus.utlc.beta.encoding.core
+import lambda_calculus.utlc.beta.encoding.nat
+
+namespace lambda_calculus
+namespace utlc
+namespace β
+namespace encoding
+namespace utlc
+
+def encode_utlc: utlc → encoded_data
+| (↓n) := alternative (show 0 < 3, by simp) (complexity.encode distance_model n)
+| (Λ f) := alternative (show 1 < 3, by simp) (encode_utlc f)
+| (f·g) := alternative (show 2 < 3, by simp) (pair (encode_utlc f) (encode_utlc g))
+
+instance: complexity.has_encoding distance_model utlc := ⟨ ⟨ encode_utlc,
+  begin
+    intros x y,
+    simp only [value_inj],
+    induction x generalizing y;
+    cases y;
+    try { { simp [encode_utlc, alternative, pair, complexity.encode, show 0 ≠ 2, by norm_num] } },
+    simp [encode_utlc, alternative, pair, complexity.encode, x_ih],
+    simp [encode_utlc, alternative, pair, complexity.encode, x_ih_f, x_ih_g],
+  end ⟩ ⟩
+
+end utlc
+end encoding
+end β
+end utlc
+end lambda_calculus
