src/lambda_calculus/utlc/beta_eta/basic.lean
@@ -1,0 +1,63 @@
+import lambda_calculus.utlc.basic
+import lambda_calculus.utlc.identities
+import lambda_calculus.utlc.reduction
+import lambda_calculus.utlc.beta.basic
+import lambda_calculus.utlc.eta.basic
+
+
+namespace lambda_calculus
+namespace utlc
+namespace βη
+
+def head_step (f g: utlc) := β.head_step f g ∨ η.head_step f g
+
+instance : has_βη_reduction utlc := ⟨ reduction_step_of head_step ⟩
+
+theorem step_iff (f g: utlc): f →βη g ↔ f →β g ∨ f →η g :=
+begin
+  induction f generalizing g;
+  simp only [lambda_notation, dot_notation, has_βη_reduction.step] at *,
+  { simp [head_step] },
+  { simp [lambda_reduction_step_iff, head_step, η.lambda_step_iff, β.lambda_step_iff, f_ih,
+      and_or_distrib_left, exists_or_distrib,
+      @or.left_comm _ (f_f = g ↑¹ 0 · ↓0)] },
+  { simp [dot_reduction_step_iff, head_step, η.dot_step_iff', β.dot_step_iff, f_ih_f, f_ih_g,
+      and_or_distrib_left, exists_or_distrib, and.assoc, or.assoc],
+    itauto }
+end
+
+theorem reduction_of_beta {f g: utlc}: f ↠β g → f ↠βη g :=
+begin
+  intro p,
+  induction p with x g hfx hxg ih,
+  refl,
+  apply trans ih (relation.refl_trans_gen.single _),
+  rw [step_iff],
+  exact or.inl hxg,
+end
+
+theorem reduction_of_eta {f g: utlc}: f ↠η g → f ↠βη g :=
+begin
+  intro p,
+  induction p with x g hfx hxg ih,
+  refl,
+  apply trans ih (relation.refl_trans_gen.single _),
+  rw [step_iff],
+  exact or.inr hxg,
+end
+
+def head_reduced (f: utlc): bool := β.head_reduced f ∧ η.head_reduced f
+
+def reduced := reduced_of head_reduced
+
+theorem reduced_iff_no_reduction {f: utlc}: reduced f ↔ ∀ g, ¬ f →βη g :=
+begin
+  apply reduced_iff_not_reduction_step,
+  intro f,
+  simp [head_reduced, head_step, β.not_head_step_iff_head_reduced, η.head_reduced_iff_not_head_step,
+    forall_and_distrib, not_or_distrib],
+end 
+
+end βη
+end utlc
+end lambda_calculus
