src/lambda_calculus/utlc/beta_eta/church_rosser.lean
@@ -1,0 +1,234 @@
+import lambda_calculus.utlc.basic
+import lambda_calculus.utlc.identities
+import lambda_calculus.utlc.reduction
+import lambda_calculus.utlc.beta.basic
+import lambda_calculus.utlc.beta.church_rosser
+import lambda_calculus.utlc.eta.basic
+import lambda_calculus.utlc.eta.normal
+import lambda_calculus.utlc.eta.church_rosser
+import lambda_calculus.utlc.beta_eta.basic
+import logic.relation
+
+
+namespace lambda_calculus
+namespace utlc
+namespace βη
+
+local notation a `[` b `:=` c  `]` : 70 := has_substitution.substitution a b c
+
+theorem βη_diamond_step {a b c: utlc}:
+   a →β b → a →η c →
+   ∃ x, b ↠η x ∧ (c = x ∨ c →β x) :=
+begin
+  induction a generalizing b c;
+  simp;
+  intros hab hac,
+  { rcases β.lambda_step_exists hab with ⟨b₁, hb₁, hab⟩,
+    cases η.lambda_step_cases' hac with hac hac;
+    rcases hac with ⟨c₁, hc₁, hac⟩;
+     rw [hb₁, hc₁],
+    { rcases a_ih hab hac with ⟨x, hbx, hcx⟩,
+      use Λ x,
+      refine ⟨ η.lambda_reduction_lambda hbx, _ ⟩,
+      simp [hcx] },
+    rw [hac] at hab,
+    obtain hab|hab|hab := β.dot_step_cases hab;
+    rcases hab with ⟨b₂, hab , hb₂⟩,
+    { 
+      cases shift_of_uses (show b₂.uses 1 = 0, begin
+        rw [← lambda_uses, ← hab],
+        exact shift_uses_zero _,
+      end) with b₃ hb₃,
+      rw [hb₃, ← lambda_shift, shift_inj_iff] at hab,
+      rw [hab, ←hb₂, hb₃, shift_succ_substitiution_down],
+      use Λ b₃,
+      exact ⟨ by refl, or.inl rfl⟩ },
+    { rw [hab],
+      cases shift_of_uses (β.uses_zero_step hb₂ (shift_uses_zero _)) with b₃ hb₃,
+      rw [hb₃],
+      rw [hb₃] at hb₂,
+      use b₃,
+      split,
+      apply relation.refl_trans_gen.single,
+      apply η.lambda_step_head,
+      right,
+      apply (shift_reduction_step_shift_iff _).mp,
+      apply hb₂,
+      apply β.shift_head_step_shift },
+    { simp at hb₂, contradiction } },
+  { obtain hab|hab|hab := β.dot_step_cases hab;
+    cases η.dot_step_cases' hac with hac hac;
+    rcases hab with ⟨x, hax, hxb⟩;
+    rcases hac with ⟨y, z, hza, hcyz, hay⟩,
+    { rw [←hxb, ←hza, hcyz],
+      rw [hax] at hay,
+      cases η.lambda_step_cases' hay with hay hay;
+      rcases hay with ⟨y₁, hy₁, hxy₁⟩,
+      { rw [hy₁],
+        use y₁[0:=z],
+        split,
+        apply substitution_reduction_step_left,
+        apply η.head_step_substitution,
+        apply hxy₁,
+        right,
+        apply β.lambda_dot_step_substitution },
+      { simp [hxy₁, hy₁],
+        use y₁·z,
+        exact ⟨by refl, or.inl rfl⟩ } },
+    { rw [← hxb, hcyz, hza, hax],
+      use x[0:=z],
+      split,
+      apply substitution_reduction_step_right,
+      apply η.shift_head_step_shift,
+      apply hay,
+      right,
+      apply β.lambda_dot_step_substitution, },
+    { rw [hax, ← hza, hcyz],
+      rcases a_ih_f hxb hay with ⟨m, hxm, hym⟩,
+      use m·z,
+      split,
+      apply η.dot_reduction_dot_left hxm,
+      cases hym,
+      { simp [hym] },
+      right,
+      apply β.dot_step_dot_left hym },
+    { rw [hax, hcyz, hza],
+      use x·z,
+      split,
+      apply η.dot_reduction_dot_right,
+      apply relation.refl_trans_gen.single hay,
+      right,
+      apply β.dot_step_dot_left hxb },
+    { rw [hax, hcyz, hza],
+      use y·x,
+      split,
+      apply η.dot_reduction_dot_left,
+      apply relation.refl_trans_gen.single hay,
+      right,
+      apply β.dot_step_dot_right hxb },
+    { rw [hax, ← hza, hcyz],
+      rcases a_ih_g hxb hay with ⟨m, hxm, hym⟩,
+      use y·m,
+      split,
+      apply η.dot_reduction_dot_right hxm,
+      cases hym,
+      { simp [hym] },
+      right,
+      apply β.dot_step_dot_right hym }
+  }
+end
+
+theorem βη_diamond_step_reduction {a b c: utlc}: a →β b → a ↠η c →
+  ∃ x, b ↠η x ∧ c ↠β x :=
+begin
+  intros hab hac,
+  induction hac using relation.refl_trans_gen.head_induction_on with a f haf hfc ih generalizing b hab,
+  exact ⟨b, by refl, relation.refl_trans_gen.single hab ⟩,
+  rcases βη_diamond_step hab haf with ⟨g, hbg, hfg⟩,
+  cases hfg,
+  { refine ⟨ c, trans hbg _, by refl ⟩,
+    rw [← hfg],
+    exact hfc },
+  rcases ih hfg with ⟨x, hgx, hcx⟩,
+  refine ⟨x, trans hbg hgx, hcx⟩,
+end
+
+theorem βη_diamond_reduction {a b c: utlc}: a ↠β b → a ↠η c →
+  ∃ x, b ↠η x ∧ c ↠β x :=
+begin
+  intros hab hac,
+  induction hab using relation.refl_trans_gen.head_induction_on with a f haf hfb ih generalizing c hac,
+  exact ⟨c, hac, by refl⟩,
+  rcases βη_diamond_step_reduction haf hac with ⟨g, hfg, hcg⟩,
+  rcases ih hfg with ⟨x, hbx, hgx⟩,
+  refine ⟨x, hbx, trans hcg hgx⟩,
+end
+
+theorem β_diamond_reduction {a b c: utlc}: a ↠β b → a ↠βη c →
+  ∃ x, b ↠βη x ∧ c ↠β x :=
+begin
+  intros hab hac,
+  induction hac using relation.refl_trans_gen.head_induction_on with a f haf hfc ih generalizing b hab,
+  exact ⟨b, by refl, hab⟩,
+  rw [step_iff] at haf,
+  cases haf,
+  { rcases β.church_rosser hab (relation.refl_trans_gen.single haf) with ⟨x, hbx, hfx⟩,
+    rcases ih hfx with ⟨y, hxy, hcy⟩,
+    refine ⟨y, trans (reduction_of_beta hbx) hxy, hcy⟩ },
+  { rcases βη_diamond_reduction hab (relation.refl_trans_gen.single haf) with ⟨x, hbx, hfx⟩,
+    rcases ih hfx with ⟨y, hxy, hcy⟩,
+    refine ⟨y, trans (reduction_of_eta hbx) hxy, hcy⟩ },
+end
+
+theorem η_diamond_reduction {a b c: utlc}: a ↠η b → a ↠βη c →
+  ∃ x, b ↠βη x ∧ c ↠η x :=
+begin
+  intros hab hac,
+  induction hac using relation.refl_trans_gen.head_induction_on with a f haf hfc ih generalizing b hab,
+  exact ⟨b, by refl, hab⟩,
+  rw [step_iff] at haf,
+  cases haf,
+  { rcases βη_diamond_reduction (relation.refl_trans_gen.single haf) hab with ⟨x, hfx, hbx⟩,
+    rcases ih hfx with ⟨y, hxy, hcy⟩,
+    refine ⟨y, trans (reduction_of_beta hbx) hxy, hcy⟩ },
+  { rcases η.church_rosser hab (relation.refl_trans_gen.single haf) with ⟨x, hbx, hfx⟩,
+    rcases ih hfx with ⟨y, hxy, hcy⟩,
+    refine ⟨y, trans (reduction_of_eta hbx) hxy, hcy⟩ }
+end
+
+theorem church_rosser {a b c : utlc}:
+  a ↠βη b → a ↠βη c → b ≡βη c :=
+begin
+  intros hab hac,
+  induction hab using relation.refl_trans_gen.head_induction_on with a f haf hfb ih generalizing c hac,
+  { use c,
+    exact ⟨ hac, by refl⟩, },
+  rw [step_iff] at haf,
+  cases haf,
+  { rcases β_diamond_reduction (relation.refl_trans_gen.single haf) hac with ⟨x, hfx, hcx⟩,
+    rcases ih hfx with ⟨y, hby, hxy⟩,
+    refine ⟨y, hby, trans (reduction_of_beta hcx) hxy ⟩ },
+  { rcases η_diamond_reduction (relation.refl_trans_gen.single haf) hac with ⟨x, hfx, hcx⟩,
+    rcases ih hfx with ⟨y, hby, hxy⟩,
+    refine ⟨y, hby, trans (reduction_of_eta hcx) hxy ⟩ }
+end
+
+
+@[refl]
+theorem equiv_refl (f : utlc): f ≡βη f :=
+  ⟨f, relation.refl_trans_gen.refl, relation.refl_trans_gen.refl⟩
+
+@[symm]
+theorem equiv_symm {a b: utlc}: a ≡βη b → b ≡βη a :=
+begin
+  apply relation.symmetric_join
+end
+
+@[trans]
+theorem equiv_trans {a b c : utlc}: a ≡βη b → b ≡βη c → a ≡βη c :=
+begin
+  apply relation.transitive_join,
+  apply relation.refl_trans_gen.trans,
+  apply @church_rosser,
+end
+
+theorem reduced_reduction_inj {f g: utlc}: reduced f → f ↠βη g → f = g :=
+begin
+  intros hf p,
+  induction p with x y hx hy fx,
+  { refl },
+  rw [←fx] at *,
+  exfalso,
+  apply reduced_iff_no_reduction.mp hf _ hy
+end
+
+theorem reduced_equiv_inj {f g: utlc}: reduced f → reduced g → f ≡βη g → f = g :=
+begin
+  intros hf hg p,
+  cases p with x p,
+  rw [reduced_reduction_inj hf p.left, reduced_reduction_inj hg p.right]
+end
+
+end βη
+end utlc
+end lambda_calculus
