src/lambda_calculus/utlc/complexity/instance.lean
@@ -1,0 +1,57 @@
+import lambda_calculus.utlc.complexity.basic
+
+namespace lambda_calculus
+namespace complexity
+
+open complexity.complexity_le
+open utlc
+
+structure is_complexity {α: Type} [has_encodable_function α] (f: α):=
+mk :: (cost : cost_function' α) (inv : complexity_le f cost)
+
+class has_complexity {α: Type} [has_encodable_function α] (f: α) :=
+  (value: is_complexity f)
+
+def complexity {α: Type} [has_encodable_function α]  (f: α) [cf: has_complexity f] := 
+  cf.value.1
+
+instance value_complexity (α: Type) [has_encoding α] (a: α): has_complexity a :=
+  ⟨ ⟨ (0:ℕ), (value_complexity_le _) ⟩ ⟩
+
+instance compose_complexity (α β γ: Type) [α_en: has_encoding α] [β_en: has_encoding β] [γ_en: has_encodable_function γ]
+  (f: α → β) (g: β → γ) [cf: has_complexity f] [cg: has_complexity g] : has_complexity (g∘f) :=
+begin
+  fconstructor,
+  fconstructor,
+  swap,
+  apply compose_complexity_le β _ cf.value.2 cg.value.2,
+  refl,
+  { intro a, refl },
+end
+
+instance iteration_complexity (α: Type) [α_en: has_encoding α]
+  (f: α → α) [cf: has_complexity f]: has_complexity (nat.iterate f) :=
+begin
+  fconstructor,
+  fconstructor,
+  swap,
+  apply iteration_complexity_le,
+  apply cf.value.2,
+  refl,
+  { intros a b, refl },
+end
+
+instance flip_complexity (α β γ: Type) [α_en: has_encoding α] [β_en: has_encoding β] [γ_en: has_encoding γ]
+  (f: α → β → γ) [cf: has_complexity f]: has_complexity (flip f) :=
+begin
+  fconstructor,
+  fconstructor,
+  swap,
+  apply flip_complexity_le,
+  apply cf.value.2,
+  refl,
+  { intros a b, refl },
+end
+
+end complexity
+end lambda_calculus
