src/lambda_calculus/utlc/eta/basic.lean
@@ -1,0 +1,373 @@
+import lambda_calculus.notation
+import lambda_calculus.utlc.basic
+import lambda_calculus.utlc.identities
+import lambda_calculus.utlc.reduction
+import logic.relation
+
+namespace lambda_calculus
+namespace utlc
+namespace η
+
+local notation a `[` b `:=` c  `]` : 70 := has_substitution.substitution a b c
+
+variables {f g f' g' x y z: utlc}
+
+@[simp]
+def head_step : utlc → utlc → Prop := λ f g, f = Λ (g ↑¹ 0)·↓0
+
+instance : has_η_reduction utlc := ⟨ reduction_step_of head_step ⟩
+
+@[simp] theorem down_step {n: ℕ}: ¬ ↓n →η g :=
+begin
+  simp [has_η_reduction.step, reduction_step],
+end
+
+theorem lambda_step_lambda : f →η g → (Λ f) →η (Λ g) :=
+begin
+  intro p,
+  simp [has_η_reduction.step, reduction_step],
+  exact or.inr p
+end
+
+theorem lambda_step_head (f: utlc): Λ (f ↑¹ 0)·↓0 →η f :=
+by simp [has_η_reduction.step, reduction_step]
+
+theorem lambda_step_head': f = (g ↑¹ 0)·↓0 → Λ f →η g :=
+by { intro p, rw[p], exact lambda_step_head _ }
+
+theorem lambda_step_iff: Λ f →η g ↔ (∃ x, g = x ∧ f = (x ↑¹ 0)·↓0) ∨ (∃ x, g = Λ x ∧ f →η x) :=
+by simp [has_η_reduction.step, reduction_step]
+
+theorem lambda_step_cases : Λ f →η g → (∃ x, g = Λ x ∧ f →η x ∨ g = x ∧ f = (x ↑¹ 0)·↓0) :=
+begin
+  simp [has_η_reduction.step, reduction_step],
+  intro p,
+  cases p,
+  use g,
+  exact or.inr ⟨rfl, p⟩,
+  cases g,
+  all_goals { simp [has_η_reduction.step, reduction_step] at * },
+  any_goals { contradiction },
+  use g,
+  exact or.inl ⟨rfl, p⟩,  
+end
+
+theorem lambda_step_cases': Λ f →η g → (∃ x, g = Λ x ∧ f →η x) ∨ ∃ x, g = x ∧ f = (x ↑¹ 0)·↓0 :=
+begin
+  intro p,
+  cases lambda_step_cases p,
+  cases h,
+  left,
+  use w,
+  assumption,
+  right,
+  use w,
+  assumption,
+end
+
+theorem dot_step_dot_left : f →η f' → (f·g) →η (f'·g) :=
+begin
+  intro p,
+  simp [has_η_reduction.step, reduction_step],
+  exact or.inl p,
+end
+
+theorem dot_step_dot_right : g →η g' → (f·g) →η (f·g') :=
+begin
+  intro p,
+  simp [has_η_reduction.step, reduction_step],
+  exact or.inr p,
+end
+
+theorem dot_step_iff: (f·f') →η g ↔ ∃ x x', g = x·x' ∧ (x' = f' ∧ f →η x ∨ x = f ∧ f' →η x') :=
+begin
+  cases g,
+  all_goals { simp [has_η_reduction.step, and_assoc] },
+end
+
+theorem dot_step_iff': (f·f') →η g ↔ (∃ x x', x' = f' ∧ g = x·x' ∧ f →η x) ∨ (∃ x x', x = f ∧ g = x·x' ∧ f' →η x') :=
+begin
+  cases g,
+  all_goals { simp [has_η_reduction.step, and_assoc] },
+end
+
+theorem dot_step_cases: (f·f') →η g → ∃ x x', g = x·x' ∧ (x' = f' ∧ f →η x ∨ x = f ∧ f' →η x') :=
+begin
+  cases g,
+  all_goals { simp [has_η_reduction.step, and_assoc] },
+end
+
+theorem dot_step_cases': (f·f') →η g → (∃ x x', x' = f' ∧ g = x·x' ∧ f →η x) ∨ (∃ x x', x = f ∧ g = x·x' ∧ f' →η x') :=
+begin
+  cases g,
+  all_goals { simp [has_η_reduction.step, and_assoc] },
+end
+
+
+theorem reduction_step_shift (n: ℕ): f ↑¹ n →η g ↑¹ n → f →η g :=
+begin
+  induction f generalizing g n,
+  { simp },
+  { simp,
+    intro p,
+    cases lambda_step_cases p with x p,
+    cases p with p p,
+    { cases p with hgx hfx,
+      have h: (g ↑¹ n).uses n = x.uses (n + 1),
+      { simp [hgx, uses] },
+      have h: ∃ y, x = y ↑¹ (n+1),
+      { apply shift_of_uses,
+        rw [← h],
+        simp [shift_uses] },
+      cases h with y hy,
+      rw [hy,
+          ← show (Λ y) ↑¹ n = Λ y ↑¹ (n+1), by simp,
+          shift_inj_iff] at hgx,
+      rw [hgx],
+      apply lambda_step_lambda,
+      apply f_ih,
+      rw [← hy],
+      apply hfx },
+    { cases p with hgx hfx,
+      -- rw [← hgx, ← shift_comm] at hfx,
+      apply lambda_step_head',
+      rw [← shift_inj_iff (n + 1), hfx],
+      simp,
+      rw [shift_comm, hgx],
+      apply nat.zero_le } },
+  { simp,
+    intro p,
+    cases g;
+    try { simp[has_η_reduction.step, reduction_step] at p,
+      contradiction },
+    rcases dot_step_cases p with ⟨x, y, hgxy, p⟩,
+    simp at hgxy,
+    simp,
+    cases p with p p,
+    cases p with hfy hfx,
+    simp [hfy] at hgxy,
+    rw [hgxy.right],
+    rw [← hgxy.left] at hfx,
+    exact dot_step_dot_left (f_ih_f _ hfx),
+    cases p with hfx hfy,
+    simp [hfx] at hgxy,
+    rw [hgxy.left],
+    rw [← hgxy.right] at hfy,
+    exact dot_step_dot_right (f_ih_g _ hfy) }
+end
+
+theorem reduction_step_uses: f →η g → ∀ n, f.uses n = g.uses n :=
+begin
+  induction f generalizing g,
+  { all_goals { simp } },
+  { intros p n,
+    cases lambda_step_cases p with x p,
+    cases p with p p,
+    { simp [uses, p.left], exact f_ih p.right _},
+    { simp [uses, p, show 0 ≠ n + 1, by linarith],
+      rw [shift_uses_lt, nat.add_sub_cancel],
+      exact nat.zero_lt_succ _ } },
+  {
+    intros p m,
+    rcases dot_step_cases p with ⟨x, y, hg, p⟩,
+    cases p with p p,
+    { simp [p.left, hg, uses],
+      apply f_ih_f p.right },
+    { simp [p.left, hg, uses],
+      apply f_ih_g p.right } }
+end
+
+theorem reduction_step_size: f →η g → f.size = g.size + 3 :=
+begin
+  induction f generalizing g;
+  simp,
+  simp [lambda_step_iff],
+  intro p,
+  cases p,
+  { rw [p], simp },
+  { rcases p with ⟨x, hgx, hfx⟩,
+    simp [f_ih hfx, hgx] },
+  { intro p,
+    rcases dot_step_cases p with ⟨x, y, hgxy, p⟩,
+    cases p with p p;
+    rcases p with ⟨heq, hstep⟩,
+    simp [f_ih_f hstep, hgxy, ← heq],
+    ring,
+    simp [f_ih_g hstep, hgxy, ← heq],
+    ring,
+  }
+end
+
+theorem reduction_step_size_mono: f →η g → g.size < f.size :=
+by intro p; simp [reduction_step_size p]
+
+@[simp] theorem down_reduction_iff {n: ℕ}: ↓n ↠η g ↔ g = ↓n :=
+begin
+  split;
+  intro p,
+  cases relation.refl_trans_gen.cases_head p,
+  { apply h.symm },
+  { simp at h, contradiction },
+  rw [p],
+end
+
+theorem lambda_reduction_lambda: f ↠η f' → Λ f ↠η Λ f' :=
+begin
+  intro p,
+  induction p,
+  { refl },
+  apply relation.refl_trans_gen.tail,
+  assumption,
+  apply lambda_step_lambda,
+  assumption,
+end
+
+theorem dot_reduction_dot_left: f ↠η f' → f·g ↠η f'·g :=
+begin
+  intro p,
+  induction p,
+  { refl },
+  apply relation.refl_trans_gen.tail,
+  assumption,
+  apply dot_step_dot_left,
+  assumption,
+end
+
+theorem dot_reduction_dot_right: g ↠η g' → f·g ↠η f·g' :=
+begin
+  intro p,
+  induction p,
+  { refl },
+  apply relation.refl_trans_gen.tail,
+  assumption,
+  apply dot_step_dot_right,
+  assumption,
+end
+
+theorem dot_reduction_dot: f ↠η f' → g ↠η g' → f·g ↠η f'·g' :=
+begin
+  intros p q,
+  apply trans,
+  apply dot_reduction_dot_left,
+  assumption,
+  apply dot_reduction_dot_right,
+  assumption,
+end
+
+theorem dot_exists_reduction (h: f ↠η g): ∀ {m n}, f = m·n → ∃ x y, g = x·y ∧ m ↠η x ∧ n ↠η y :=
+begin
+  induction h using relation.refl_trans_gen.head_induction_on with f f' hf hfg ih,
+  { intros m n p,
+    refine ⟨ m, n, p, by refl, by refl⟩ },
+  { intros m n p,
+    rw [p] at hf,
+    rcases dot_step_cases hf with ⟨a, b, hab, h⟩,
+    rcases ih hab with ⟨i, j, ih⟩,
+    refine ⟨i, j, ih.left, trans _ ih.right.left, trans _ ih.right.right⟩;
+    cases h;
+    try { simp[h] };
+    cases h;
+    try { apply relation.refl_trans_gen.single, assumption } }
+end
+
+theorem dot_reduction_cases (h: f·f' ↠η g): ∃ x y, g = x·y ∧ f ↠η x ∧ f' ↠η y := dot_exists_reduction h rfl
+
+theorem dot_reduction_dot_iff: f·g ↠η f'·g' ↔ f ↠η f' ∧ g ↠η g' :=
+begin
+  split,
+  { intro p,
+    have h := dot_exists_reduction p rfl,
+    simp [and.assoc] at h,
+    assumption },
+  intro p,
+  apply dot_reduction_dot p.left p.right,
+end
+
+theorem shift_head_step_shift {n: ℕ}: head_step (f ↑¹ n) (g ↑¹ n) ↔ head_step f g :=
+begin
+  cases f;
+  cases g;
+  try { simp };
+  cases f;
+  simp;
+  cases f_f;
+  cases f_g;
+  simp;
+  split_ifs;
+  simp;
+  try { simp [← @shift_comm 1 (n + 1) _ (by linarith)] };
+  try { simp [← @shift_comm 0 n _ (by linarith)] };
+  repeat { intro };
+  try { linarith };
+  split;
+  intro;
+  linarith
+end
+
+theorem head_step_substitution: head_step f f' → ∀ n g, f[n:=g] ↠η f'[n:=g]  :=
+begin
+  simp only [head_step],
+  intros p n g,
+  simp [p,
+    ← substitution_shift_ge _ _ (nat.zero_le _),
+    relation.refl_trans_gen.single (lambda_step_head _)]
+end
+
+def head_reduced : utlc → bool
+| (↓ _):= true
+| (Λ f) := match f with
+  | (↓ _) := true
+  | (Λ _) := true
+  | (f·g) := f.uses 0 > 0 ∨ g ≠ ↓0
+  end
+| (_·_) := true
+
+def reduced := reduced_of head_reduced
+
+theorem head_reduced_iff_not_head_step: head_reduced f ↔ ∀ g, ¬ head_step f g :=
+begin
+  cases f;
+  try { cases f };
+  simp[head_reduced],
+  split,
+  { intros p g q,
+    cases p,
+    exfalso,
+    apply (ne_of_lt p).symm,
+    rw [q],
+    apply shift_uses_zero,
+    assumption },
+  intros p,
+  obtain h|h|h := nat.lt_trichotomy (f_f.uses 0) 0,
+  { simp at h, contradiction },
+  { cases shift_of_uses h with g h,
+    right,
+    apply p g h },
+  { left, apply h },
+end
+
+theorem reduced_iff_not_reduction (f: utlc): reduced f ↔ ∀ g, ¬ f →η g :=
+  reduced_iff_not_reduction_step @head_reduced_iff_not_head_step _
+
+
+@[simp] theorem down_reduced (n: ℕ): reduced ↓n := by simp [reduced, head_reduced, down_reduced]
+
+theorem lambda_reduced (f: utlc): reduced (Λ f) ↔ head_reduced (Λ f) ∧ reduced f :=
+by simp [reduced, head_reduced, lambda_reduced]
+
+@[simp] theorem dot_reduced (f g: utlc): reduced (f·g) ↔ reduced f ∧ reduced g := by simp [reduced, head_reduced, dot_reduced]
+
+-- inductive hypothesis useful when dealing with η reductions
+-- splits (Λ f·↓0) up to handle the (Λ f)·g ⇔ f[0:=g] case
+-- theorem η_induction_on (p: utlc → Prop): Π (f: utlc)
+--   (down: Π n, p ↓n)
+--   (dot_lambda: Π x (hx: p x) (h: x.uses 0 = 0), p (Λ x·↓0))
+--   (lambda: Π x (hx: p x) (h: head_reduced x), p (Λ x))
+--   (dot : Π x y (hx: p x) (hy: p y), p (x·y)),
+--   (p f)
+-- | (↓n) := λ hn hx hdx hlx, hn n
+-- | (Λ x) := λ hn hx hdx hlx, hx x (β_induction_on x hn hx hdx hlx)
+
+end η
+end utlc
+end lambda_calculus
