src/lambda_calculus/utlc/eta/church_rosser.lean
@@ -1,0 +1,137 @@
+import lambda_calculus.utlc.basic
+import lambda_calculus.utlc.reduction
+import lambda_calculus.utlc.eta.basic
+import logic.relation
+
+namespace lambda_calculus
+namespace utlc
+namespace η
+
+theorem step_church_rosser {a b c :utlc}: a →η b → a →η c →
+  ∃ d, relation.refl_gen has_η_reduction.step b d
+    ∧ c ↠η d :=
+begin
+  induction a generalizing b c,
+  all_goals { simp },
+  { intros hab hac,
+    cases lambda_step_cases hab with x hab,
+    cases hab with hab hab,
+    all_goals { cases lambda_step_cases hac with y hac },
+    all_goals { cases hac with hac hac },
+    { cases a_ih hab.right hac.right with z ih,
+      use Λ z,
+      rw [hab.left, hac.left],
+      refine ⟨ lambda_refl_reduction_step_lambda ih.left, lambda_reduction_lambda ih.right ⟩ },
+    { rw [hab.left, hac.left],
+      rw [hac.right] at hab,
+      cases x,
+      all_goals { simp [has_η_reduction.step, and_assoc] at hab },
+      any_goals { contradiction },
+      simp,
+      have h: x_f.uses 0 = 0,
+      { rw [← reduction_step_uses hab.right.right, shift_uses_zero] },
+      cases shift_of_uses h with x' hx,
+      use x',
+      rw [hab.right.left, hx],
+      split,
+      apply relation.refl_gen.single,
+      apply lambda_step_head,
+      apply relation.refl_trans_gen.single,
+      apply reduction_step_shift 0,
+      rw [← hx],
+      apply hab.right.right },
+    { rw [hab.left, hac.left],
+      rw [hab.right] at hac,
+      cases y,
+      all_goals { simp [has_η_reduction.step, and_assoc] at hac },
+      any_goals { contradiction },
+      simp,
+      have h: y_f.uses 0 = 0,
+      { rw [← reduction_step_uses hac.right.right, shift_uses_zero] },
+      cases shift_of_uses h with y' hy,
+      use y',
+      rw [hac.right.left, hy],
+      split,
+      apply relation.refl_gen.single,
+      apply reduction_step_shift 0,
+      rw [← hy],
+      apply hac.right.right,
+      apply relation.refl_trans_gen.single,
+      apply lambda_step_head },
+    { simp [hac.right, ← hac.left] at hab,
+      use x,
+      simp [hab],
+      exact ⟨ by refl, by refl ⟩ } },
+  { intros hab hac,
+    rcases dot_step_cases hab with ⟨x, y, bxy, hab⟩,
+    cases hab with hab hab,
+    all_goals { rcases dot_step_cases hac with ⟨x', y', cxy, hac⟩ },
+    all_goals { cases hac with hac hac },
+    { cases a_ih_f hab.right hac.right with d ih,
+      use d·y,
+      rw [bxy, cxy, hac.left, ← hab.left],
+      refine ⟨ dot_refl_reduction_step_dot_left ih.left _, dot_reduction_dot_left ih.right ⟩
+    },
+    { use x·y',
+      rw [bxy, cxy, hab.left, hac.left],
+      refine ⟨ dot_refl_reduction_step_dot_right _ _, dot_reduction_dot_left _ ⟩,
+      apply relation.refl_gen.single,
+      apply hac.right,
+      apply relation.refl_trans_gen.single,
+      apply hab.right },
+    { use x'·y,
+      rw [bxy, cxy, hab.left, hac.left],
+      refine ⟨ dot_refl_reduction_step_dot_left _ _, dot_reduction_dot_right _ ⟩,
+      apply relation.refl_gen.single,
+      apply hac.right,
+      apply relation.refl_trans_gen.single,
+      apply hab.right },
+    { cases a_ih_g hab.right hac.right with d ih,
+      use x·d,
+      rw [bxy, cxy, hac.left, hab.left],
+      refine ⟨ dot_refl_reduction_step_dot_right ih.left _, dot_reduction_dot_right ih.right ⟩
+    }
+  }
+end
+
+theorem church_rosser {a b c :utlc}: a ↠η b → a ↠η c → b ≡η c :=
+  relation.church_rosser @step_church_rosser
+
+@[refl]
+theorem equiv_refl (f : utlc): f ≡η f :=
+  ⟨f, relation.refl_trans_gen.refl, relation.refl_trans_gen.refl⟩
+
+@[symm]
+theorem equiv_symm {a b: utlc}: a ≡η b → b ≡η a :=
+begin
+  apply relation.symmetric_join
+end
+
+@[trans]
+theorem equiv_trans {a b c : utlc}: a ≡η b → b ≡η c → a ≡η c :=
+begin
+  apply relation.transitive_join,
+  apply relation.refl_trans_gen.trans,
+  apply @church_rosser,
+end
+
+theorem reduced_reduction_inj {f g: utlc}: reduced f → f ↠η g → f = g :=
+begin
+  intros hf p,
+  induction p with x y hx hy fx,
+  { refl },
+  rw [←fx] at *,
+  exfalso,
+  apply (reduced_iff_not_reduction _).mp hf _ hy
+end
+
+theorem reduced_equiv_inj {f g: utlc}: reduced f → reduced g → f ≡η g → f = g :=
+begin
+  intros hf hg p,
+  cases p with x p,
+  rw [reduced_reduction_inj hf p.left, reduced_reduction_inj hg p.right]
+end
+
+end η
+end utlc
+end lambda_calculus
