src/lambda_calculus/utlc/eta/normal.lean
@@ -1,0 +1,99 @@
+import lambda_calculus.utlc.basic
+import lambda_calculus.utlc.reduction
+import lambda_calculus.utlc.eta.basic
+import logic.relation
+
+namespace lambda_calculus
+namespace utlc
+namespace η
+
+lemma normal_form_exists_helper: Π (n: ℕ), ∀ {f:utlc}, f.size ≤ n → ∃ g, f ↠η g ∧ reduced g
+| (0) := begin
+  intros f p,
+  exfalso,
+  linarith [size_pos f]
+end
+| (n+1) := begin
+  intros f p,
+  apply dite (reduced f),
+  { intro q, exact ⟨f, by refl, q⟩ },
+  rw [reduced_iff_not_reduction],
+  simp,
+  intros x fx,
+  rcases normal_form_exists_helper n (nat.le_of_lt_succ (lt_of_lt_of_le (reduction_step_size_mono fx) p)) with ⟨y, hxy, hy⟩,
+  exact ⟨y, relation.refl_trans_gen.head fx hxy, hy⟩,
+end
+
+theorem normal_form_exists (f: utlc): ∃ g, f ↠η g ∧ reduced g := normal_form_exists_helper f.size (le_refl _)
+
+-- def normal_form: utlc → utlc
+-- | (↓n) := ↓n
+-- | (Λ (↓n)) := (Λ (↓n))
+-- | (Λ (Λ f)) := Λ normal_form (Λ f)
+-- | (Λ (f·g)) := if f.uses 0 = 0 ∧ g = ↓0
+--   then normal_form f
+--   else Λ normal_form f · normal_form g
+-- | (f·g) := (normal_form f) · (normal_form g)
+
+-- theorem blah (f g: utlc): head_reduced f → f ↠η g → head_reduced g :=
+-- begin
+--   induction f generalizing g,
+--   { simp, intros _ p, rw[p], simp[head_reduced] },
+--   { simp,
+--     intros p q,
+--     revert p,
+--     induction q with x g hfx hxg,
+--     simp,
+--     intro p,
+--     specialize q_ih p,
+--     cases x,
+--     { simp at hxg, contradiction },
+--     swap,
+--     { simp [dot_step_iff] at hxg,
+--       rcases hxg with ⟨_, _, h, _⟩,
+--       simp [h, head_reduced] },
+--     simp at *,
+--     cases x,
+--     { simp[lambda_step_iff] at hxg, contradiction },
+--     { rw [lambda_step_iff] at hxg,
+--       simp at hxg,
+--       rcases hxg with ⟨ y, hgy, hxy ⟩,
+      
+
+--     }
+--   },
+--   { simp,
+--     intros p q,
+--     rcases dot_reduction_cases q with ⟨x, y, hgxy, _, _⟩,
+--     rw [hgxy],
+--     simp [head_reduced],
+--   }
+-- end
+
+-- def normal_form_exists (f: utlc): ∃ g, f ↠η g ∧ reduced g :=
+-- begin
+--   induction f,
+--   { use f, simp },
+--   { apply dite (head_reduced (Λ f_f)),
+--     intro p,
+--     cases f_ih with g h,
+--     use Λ g,
+--     refine ⟨ lambda_reduction_lambda h.left, _⟩,
+--     rw [lambda_reduced], 
+--     refine ⟨_, h.right⟩,
+
+    
+
+--   },
+--   { cases f_ih_f with x hx,
+--     cases f_ih_g with y hy,
+--     use x·y,
+--     split,
+--     apply dot_reduction_dot hx.left hy.left,
+--     simp,
+--     exact ⟨hx.right, hy.right⟩ }
+-- end
+
+end η
+end utlc
+end lambda_calculus
